ARCH2022_Examples.thy
@@ -1,0 +1,1796 @@
+(*  Title:       Examples of hybrid systems verifications
+    Author:      Jonathan Julián Huerta y Munive, 2020
+    Maintainer:  Jonathan Julián Huerta y Munive <jonjulian23@gmail.com>
+*)
+
+section \<open> Examples \<close>
+
+text \<open> We prove partial correctness specifications of some hybrid systems with our 
+verification components.\<close>
+
+theory ARCH2022_Examples
+  imports "HS_VC_Spartan"
+
+begin
+
+
+subsection \<open> Basic \<close>
+
+
+subsubsection \<open> Basic assignment \<close> 
+
+(* x>=0 -> [x:=x+1;]x>=1 *)
+lemma "(\<lambda>s. s$1 \<ge> (0::real)) \<le> |1 ::= (\<lambda>s. s$1 +1)] (\<lambda>s. s$1 \<ge> 1)"
+  by simp
+
+
+subsubsection \<open> Overwrite assignment on some branches \<close>
+
+(* x>=0 -> [x:=x+1;][x:=x+1; ++ y:=x+1;]x>=1 *)
+lemma "(\<lambda>s. s$1 \<ge> (0::real)) \<le> |1 ::= (\<lambda>s. s$1 +1)] 
+  |(\<lambda>s. (1 ::= (\<lambda>s. s$1 +1)) s \<union> (2 ::= (\<lambda>s. s$1 +1)) s)] (\<lambda>s. s$1 \<ge> 1)"
+  by (simp add: fbox_choice le_fun_def)
+
+
+subsubsection \<open> Overwrite assignment in loop \<close>
+
+(* x>=0 -> [x:=x+1;][{x:=x+1;}*@invariant(x>=1)]x>=1 *)
+lemma "(\<lambda>s. s$1 \<ge> (0::real)) \<le> |1 ::= (\<lambda>s. s$1 +1)] 
+ |LOOP (1 ::= (\<lambda>s. s$1 +1)) INV (\<lambda>s. s$1 \<ge> 1)] (\<lambda>s. s$1 \<ge> 1)"
+  apply(subst fbox_kcomp[symmetric])
+  by (rule wp_loopI_break, auto)
+
+
+subsubsection \<open> Overwrite assignment in ODE \<close>
+
+(* x>=0 -> [x:=x+1;][{x'=2}]x>=1 *)
+lemma "(\<lambda>s. s$1 \<ge> (0::real)) \<le> 
+  |1 ::= (\<lambda>s. s$1 +1)] |x\<acute>=(\<lambda>s. (\<chi> i. if i=1 then 2 else 0)) & G] 
+  (\<lambda>s. s$1 \<ge> 1)" 
+  apply(subst local_flow.fbox_g_ode_subset[where 
+        \<phi>="\<lambda>t s. (\<chi> i. if i=1 then 2*t+s$1 else s$i)" and T=UNIV])
+     apply(unfold_locales, simp_all add: local_lipschitz_def lipschitz_on_def vec_eq_iff)
+   apply(clarsimp, rule_tac x=1 in exI)+
+  by (auto intro!: poly_derivatives)
+
+
+subsubsection \<open> Overwrite with nondeterministic assignment \<close>
+
+(* x>=0 -> [x:=x+1;][x:=*; ?x>=1;]x>=1 *)
+lemma "(\<lambda>s. s$1 \<ge> (0::real)) \<le> |1 ::= (\<lambda>s. s$1 +1)] |(1 ::= ?);\<questiondown>\<lambda>s. s$1 \<ge> 1?] (\<lambda>s. s$1 \<ge> 1)" 
+  by (simp add: le_fun_def)
+
+
+subsubsection \<open> Tests and universal quantification \<close>
+
+(* x>=0 -> [x:=x+1;][?x>=2; x:=x-1; ++ ?\forall x (x>=1 -> y>=1); x:=y;]x>=1 *)
+lemma "(\<lambda>s::real^2. s$1 \<ge> 0) \<le> |1 ::= (\<lambda>s. s$1 +1)]
+  |(\<lambda>s. (\<questiondown>\<lambda>s. s$1 \<ge> 2?;(1 ::= (\<lambda>s. s$1 - 1))) s \<union> 
+    (\<questiondown>\<lambda>s. \<forall>i. s$i \<ge> 1 \<longrightarrow> s$2 \<ge> 1?;(1 ::= (\<lambda>s. s$2))) s)] 
+  (\<lambda>s. s$1 \<ge> 1)" 
+  by (auto simp: le_fun_def fbox_choice )
+
+
+subsubsection \<open> Overwrite assignment several times \<close>
+
+(* x>=0 & y>=1 -> [x:=x+1;][{x:=x+1;}*@invariant(x>=1) ++ y:=x+1;][{y'=2}][x:=y;]x>=1 *)
+lemma "(\<lambda>s::real^2. s$1 \<ge> 0 \<and> s$2 \<ge> 1) \<le> 
+  |1 ::= (\<lambda>s. s$1 +1)] 
+  |(\<lambda>s. (LOOP (1 ::= (\<lambda>s. s$1 +1)) INV (\<lambda>s. s$1 \<ge> 1)) s \<union> (2 ::= (\<lambda>s. s$1 + 1)) s)]
+  |x\<acute>=(\<lambda>s. (\<chi> i. if i=2 then 2 else 0)) & G] |1 ::= (\<lambda>s. s$2)]
+  (\<lambda>s. s$1 \<ge> 1)"
+  apply(subst local_flow.fbox_g_ode_subset[where 
+        \<phi>="\<lambda>t s. (\<chi> i. if i=2 then 2*t+s$2 else s$i)" and T=UNIV])
+   apply(unfold_locales; simp add: local_lipschitz_def lipschitz_on_def vec_eq_iff le_fun_def)
+     apply (clarsimp, rule_tac x=1 in exI, force)
+   apply(force intro!: poly_derivatives vec_eq_iff, simp)
+  apply(subst change_loopI[where I="\<lambda>s. 1 \<le> s$1 \<and> 1 \<le> s$2"])
+  apply(subst fbox_kcomp[symmetric], rule hoare_kcomp)
+     apply(subst fbox_assign[where Q="\<lambda>s. 1 \<le> s$1 \<and> 1 \<le> s$2"], simp)
+  apply(subst le_fbox_choice_iff, rule conjI)
+  by (subst fbox_loopI, auto)
+
+
+subsubsection \<open> Potentially overwrite dynamics \<close>
+
+(* x>0 & y>0 -> [{x'=5}][{x:=x+3;}*@invariant(x>0) ++ y:=x;](x>0&y>0) *)
+lemma "(\<lambda>s::real^2. s$1 > 0 \<and> s$2 > 0) \<le> 
+   |x\<acute>=(\<lambda>s. (\<chi> i. if i=1 then 5 else 0)) & G] 
+  |(\<lambda>s. (LOOP (1 ::= (\<lambda>s. s$1 + 3)) INV (\<lambda>s. 0 < s$1)) s \<union> (2 ::= (\<lambda>s. s$1)) s)] 
+  (\<lambda>s. s$1 > 0 \<and> s$2 > 0)"
+  apply(subst fbox_kcomp[symmetric])+
+  apply(rule hoare_kcomp)+
+   apply(subst local_flow.fbox_g_ode_subset[where \<phi>="\<lambda>t s. (\<chi> i. if i=1 then 5*t+s$1 else s$i)"
+        and T=UNIV and Q="\<lambda>s. s$1 > 0 \<and> s$2 > 0"]; simp?)
+   apply(unfold_locales; (simp add: local_lipschitz_def lipschitz_on_def vec_eq_iff)?)
+    apply(clarsimp, rule_tac x=1 in exI)+
+    apply (force, force intro!: poly_derivatives, force simp: le_fun_def)
+  apply(subst le_fbox_choice_iff, rule conjI)
+   apply(subst change_loopI[where I="\<lambda>s. s$1 > 0 \<and> s$2 > 0"])
+  by (rule fbox_loopI, simp_all add: le_fun_def)
+
+
+subsubsection \<open> Potentially overwrite exponential decay \<close>
+
+abbreviation po_exp_dec_f :: "real^2 \<Rightarrow> real^2" ("f")
+  where "f s \<equiv> (\<chi> i. if i=1 then -s$1 else 0)"
+
+abbreviation po_exp_dec_flow :: "real \<Rightarrow> real^2 \<Rightarrow> real^2" ("\<phi>")
+  where "\<phi> t s \<equiv> (\<chi> i. if i=1 then s$1 * exp (- t) else s$i)"
+
+lemma local_flow_exp_flow: "local_flow f UNIV UNIV \<phi>"
+  apply(unfold_locales, simp_all add: local_lipschitz_def lipschitz_on_def)
+     apply(clarsimp simp: dist_norm norm_vec_def L2_set_def, rule_tac x=1 in exI)+
+  apply(unfold UNIV_2, simp)
+  apply (metis power2_commute real_sqrt_ge_abs1)
+  by (auto intro!: poly_derivatives simp: forall_2 vec_eq_iff)
+
+(* x>0 & y>0 -> [{x'=-x}][{x:=x+3;}*@invariant(x>0) ++ y:=x;](x>0&y>0) *)
+lemma "(\<lambda>s::real^2. s$1 > 0 \<and> s$2 > 0) \<le> |x\<acute>= f & G]
+  |(\<lambda>s. (LOOP (1 ::= (\<lambda>s. s$1 + 3)) INV (\<lambda>s. 0 < s$1)) s \<union> (2 ::= (\<lambda>s. s$1)) s)] 
+  (\<lambda>s. s$1 > 0 \<and> s$2 > 0)"
+ apply(subst fbox_kcomp[symmetric], rule hoare_kcomp)
+   apply(subst local_flow.fbox_g_ode_subset[OF 
+        local_flow_exp_flow, where Q="\<lambda>s. s$1 > 0 \<and> s$2 > 0"]; simp add: le_fun_def)
+  apply(subst le_fbox_choice_iff, rule conjI)
+   apply(subst change_loopI[where I="\<lambda>s. s$1 > 0 \<and> s$2 > 0"])
+  by (rule fbox_loopI, auto)
+
+no_notation po_exp_dec_f ("f")
+        and po_exp_dec_flow ("\<phi>")
+
+
+subsubsection \<open> Dynamics: Cascaded \<close>
+
+(* x>0 -> [{x'=5};{x'=2};{x'=x}]x>0 *)
+lemma "(\<lambda>s::real^1. s$1 > 0) \<le> 
+  |(x\<acute>=(\<lambda>s. (\<chi> i. if i=1 then 5 else 0)) & G);
+      (x\<acute>=(\<lambda>s. (\<chi> i. if i=1 then 2 else 0)) & G);
+      (x\<acute>=(\<lambda>s. (\<chi> i. if i=1 then s$1 else 0)) & G)] 
+  (\<lambda>s. s$1 > 0)"
+  apply(simp, subst local_flow.fbox_g_ode_subset[where T=UNIV and \<phi>="\<lambda>t s. (\<chi> i. 5*t+s$1)"]; simp?)
+   apply(unfold_locales; (simp add: local_lipschitz_def lipschitz_on_def vec_eq_iff)?)
+    apply(clarsimp simp: dist_norm norm_vec_def L2_set_def, rule_tac x=1 in exI)+
+    apply(force, force intro!: poly_derivatives)
+  apply(subst local_flow.fbox_g_ode_subset[where T=UNIV and \<phi>="\<lambda>t s. (\<chi> i. 2*t+s$1)"]; simp?)
+   apply(unfold_locales; (simp add: local_lipschitz_def lipschitz_on_def vec_eq_iff)?)
+    apply(clarsimp simp: dist_norm norm_vec_def L2_set_def, rule_tac x=1 in exI)+
+    apply(force, force intro!: poly_derivatives)
+  apply(subst local_flow.fbox_g_ode_subset[where T=UNIV and \<phi>="\<lambda>t s. (\<chi> i. s$1 * exp t)"]; simp?)
+   apply(unfold_locales; (simp add: local_lipschitz_def lipschitz_on_def vec_eq_iff)?)
+    apply(clarsimp simp: dist_norm norm_vec_def L2_set_def, rule_tac x=1 in exI)+
+  by (force, auto intro!: poly_derivatives)
+
+
+subsubsection \<open> Dynamics: Single integrator time \<close>
+
+(* x=0->[{x'=1}]x>=0 *)
+lemma "(\<lambda>s::real^1. s$1 = 0) \<le> |x\<acute>=(\<lambda>s. (\<chi> i. 1)) & G] (\<lambda>s. s$1 \<ge> 0)"
+  apply(subst local_flow.fbox_g_ode_subset[where T=UNIV and \<phi>="\<lambda>t s. (\<chi> i. t+s$1)"]; simp?)
+  apply(unfold_locales; (simp add: local_lipschitz_def lipschitz_on_def vec_eq_iff)?)
+   apply(clarsimp simp: dist_norm norm_vec_def L2_set_def, rule_tac x=1 in exI)+
+  by (auto intro!: poly_derivatives)
+
+
+subsubsection \<open> Dynamics: Single integrator \<close>
+
+(* x>=0 & y>=0 -> [{x'=y}]x>=0 *)
+lemma "0 \<le> t \<Longrightarrow> (\<lambda>s::real^2. s$1 \<ge> 0 \<and> s$2 \<ge> 0) \<le> 
+  |x\<acute>=(\<lambda>s. (\<chi> i. if i = 1 then s$2 else 0)) & G] (\<lambda>s. s$1 \<ge> 0)"
+  apply(subst local_flow.fbox_g_ode_subset[where T=UNIV and 
+        \<phi>="\<lambda>t s. (\<chi> i. if i = 1 then s$2*t+s$1 else s$i)"]; simp?)
+  apply(unfold_locales; (simp add: local_lipschitz_def lipschitz_on_def vec_eq_iff)?)
+    apply(simp add: dist_norm norm_vec_def L2_set_def)
+   apply(clarsimp simp: dist_norm norm_vec_def L2_set_def, rule_tac x=1 in exI)+
+  unfolding UNIV_2 by (auto intro!: poly_derivatives simp: forall_2 vec_eq_iff)
+
+
+subsubsection \<open> Dynamics: Double integrator \<close>
+
+(* x>=0 & y>=0 & z>=0 -> [{x'=y,y'=z}]x>=0 *)
+lemma "(\<lambda>s::real^3. s$1 \<ge> 0 \<and> s$2 \<ge> 0 \<and> s$3 \<ge> 0) \<le> 
+  |x\<acute>=(\<lambda>s. (\<chi> i. if i = 1 then s$2 else (if i = 2 then s$3 else 0))) & G] 
+  (\<lambda>s. s$1 \<ge> 0)"
+  apply(subst local_flow.fbox_g_ode_subset[where T=UNIV and 
+        \<phi>="\<lambda>t s. (\<chi> i. if i = 1 then s$3*t\<^sup>2/2 + s$2*t +s$1 
+            else (if i = 2 then s$3*t+s$2 else s$i))"]; simp?)
+  apply(unfold_locales; (simp add: local_lipschitz_def lipschitz_on_def vec_eq_iff)?)
+   apply(clarsimp simp: dist_norm norm_vec_def L2_set_def, rule_tac x=1 in exI)+
+  unfolding UNIV_3 by (auto intro!: poly_derivatives simp: forall_3 vec_eq_iff)
+
+
+subsubsection \<open> Dynamics: Triple integrator \<close>
+
+abbreviation triple_int_f :: "real^4 \<Rightarrow> real^4" ("f")
+  where "f s \<equiv> (\<chi> i. if i = 1 then s$2 else 
+    (if i = 2 then s$3 else (if i = 3 then s$4 else (s$4)\<^sup>2)))"
+
+(* x>=0 & y>=0 & z>=0 & j>=0 -> [{x'=y,y'=z,z'=j,j'=j\<^sup>2}]x>=0 *)
+lemma "(\<lambda>s::real^4. s$1 \<ge> 0 \<and> s$2 \<ge> 0 \<and> s$3 \<ge> 0 \<and> s$4 \<ge> 0) \<le> |x\<acute>= f & G] (\<lambda>s. s$1 \<ge> 0)"
+  apply(rule_tac C="\<lambda>s. s$4 \<ge> 0" in diff_cut_rule)
+  apply(subst g_ode_inv_def[symmetric, where I="\<lambda>s. s$4 \<ge> 0"])
+   apply(rule fbox_g_odei, simp add: le_fun_def, simp)
+    apply(rule_tac \<nu>'="\<lambda>s. 0" and \<mu>'="\<lambda>s. (s$4)\<^sup>2" in diff_inv_leqI)
+    apply(force intro!: poly_derivatives simp: forall_4 open_segment_eq_real_ivl)
+  apply force
+   apply(force intro!: poly_derivatives simp: forall_4, simp add: le_fun_def)
+  apply(rule_tac C="\<lambda>s. s$3 \<ge> 0" in diff_cut_rule, simp_all)
+  apply(subst g_ode_inv_def[symmetric, where I="\<lambda>s. s$3 \<ge> 0"])
+   apply(rule fbox_g_odei, simp add: le_fun_def, simp)
+   apply(rule_tac \<nu>'="\<lambda>s. 0" and \<mu>'="\<lambda>s. (s$4)" in diff_invariant_rules(2); simp?) 
+   apply(force intro!: poly_derivatives simp: forall_4, simp add: le_fun_def)
+  apply(rule_tac C="\<lambda>s. s$2 \<ge> 0" in diff_cut_rule, simp_all)
+  apply(subst g_ode_inv_def[symmetric, where I="\<lambda>s. s$2 \<ge> 0"])
+   apply(rule fbox_g_odei, simp add: le_fun_def, simp)
+   apply(rule_tac \<nu>'="\<lambda>s. 0" and \<mu>'="\<lambda>s. (s$3)" in diff_invariant_rules(2); simp?)
+   apply(force intro!: poly_derivatives simp: forall_4, simp add: le_fun_def)
+  apply(rule_tac C="\<lambda>s. s$1 \<ge> 0" in diff_cut_rule, simp_all)
+  apply(subst g_ode_inv_def[symmetric, where I="\<lambda>s. s$1 \<ge> 0"])
+   apply(rule fbox_g_odei, simp add: le_fun_def, simp)
+   apply(rule_tac \<nu>'="\<lambda>s. 0" and \<mu>'="\<lambda>s. (s$2)" in diff_invariant_rules(2); simp?)
+    apply(force intro!: poly_derivatives simp: forall_4, simp add: le_fun_def)
+  by (rule diff_weak_rule, simp add: le_fun_def)
+
+no_notation triple_int_f ("f")
+
+
+subsubsection \<open> Dynamics: Exponential decay (1) \<close>
+
+(* x>0 -> [{x'=-x}]x>0 *)
+lemma "(\<lambda>s::real^1. s$1 > 0) \<le> |x\<acute>=(\<lambda>s. (\<chi> i. - s$1)) & G] (\<lambda>s. s$1 > 0)"
+  apply(subst local_flow.fbox_g_ode_subset[where T=UNIV and \<phi>="\<lambda>t s. (\<chi> i. s$1 * exp (- t))"]; simp?)
+  apply(unfold_locales; (simp add: local_lipschitz_def lipschitz_on_def vec_eq_iff)?)
+   apply(clarsimp simp: dist_norm norm_vec_def L2_set_def, rule_tac x=1 in exI)+
+  by (auto intro!: poly_derivatives)
+
+
+subsubsection \<open> Dynamics: Exponential decay (2) \<close>
+
+(* x>0 -> [{x'=-x+1}]x>0 *)
+lemma "(\<lambda>s::real^1. s$1 > 0) \<le> |x\<acute>=(\<lambda>s. (\<chi> i. - s$1 + 1)) & G] (\<lambda>s. s$1 > 0)"
+  apply(subst local_flow.fbox_g_ode_subset[where T=UNIV 
+        and \<phi>="\<lambda>t s. (\<chi> i. 1 - exp (- t) + s$1 * exp (- t))"]; clarsimp?)
+   apply(unfold_locales; (simp add: local_lipschitz_def lipschitz_on_def vec_eq_iff)?)
+    apply(clarsimp simp: dist_norm norm_vec_def L2_set_def, rule_tac x=1 in exI)+
+  by (auto intro!: poly_derivatives simp: field_simps) (smt exp_gt_zero mult_pos_pos one_less_exp_iff)
+
+
+subsubsection \<open> Dynamics: Exponential decay (3) \<close>
+
+(* x>0 & y>0->[{x'=-y*x}]x>0 *)
+lemma "y > 0 \<Longrightarrow> (\<lambda>s::real^1. s$1 > 0) \<le> 
+  |x\<acute>=(\<lambda>s. (\<chi> i. - y * s$1)) & G] (\<lambda>s. s$1 > 0)"
+  apply(subst local_flow.fbox_g_ode_subset[where T=UNIV 
+        and \<phi>="\<lambda>t s. (\<chi> i. s$1 * (exp (-t * y)))"]; clarsimp?)
+  apply(unfold_locales; (simp add: local_lipschitz_def lipschitz_on_def vec_eq_iff)?)
+   apply(clarsimp, rule_tac x=1 in exI)
+   apply(clarsimp simp: dist_norm norm_vec_def L2_set_def, rule_tac x="y" in exI)
+   apply (metis abs_mult abs_of_pos dist_commute dist_real_def less_eq_real_def 
+      vector_space_over_itself.scale_right_diff_distrib)
+  by (auto intro!: poly_derivatives simp: field_simps)
+
+
+subsubsection \<open> Dynamics: Exponential growth (1) \<close>
+
+(* x>=0 -> [{x'=x}]x>=0 *)
+lemma "(\<lambda>s::real^1. s$1 \<ge> 0) \<le> |x\<acute>=(\<lambda>s. (\<chi> i. s$1)) & G] (\<lambda>s. s$1 \<ge> 0)"
+  apply(subst local_flow.fbox_g_ode_subset[where T=UNIV 
+        and \<phi>="\<lambda>t s. (\<chi> i. s$1 * exp t)"]; clarsimp?)
+  apply(unfold_locales; (simp add: local_lipschitz_def lipschitz_on_def vec_eq_iff)?)
+   apply(clarsimp simp: dist_norm norm_vec_def L2_set_def, rule_tac x=1 in exI)+
+  by (auto intro!: poly_derivatives)
+
+
+subsubsection \<open> Dynamics: Exponential growth (2) \<close>
+
+(* x>=0 & y>=0 -> [{x'=y, y'=y\<^sup>2}]x>=0 *)
+lemma "(\<lambda>s::real^2. s$1 \<ge> 0 \<and> s$2 \<ge> 0) \<le> 
+  |x\<acute>=(\<lambda>s. (\<chi> i. if i=1 then s$2 else (s$2)\<^sup>2)) & G] (\<lambda>s. s$1 \<ge> 0)"
+  apply(rule_tac C="\<lambda>s. s$2 \<ge> 0" in diff_cut_rule)
+   apply(subst g_ode_inv_def[symmetric, where I="\<lambda>s. s$2 \<ge> 0"])
+   apply(rule fbox_g_odei, simp add: le_fun_def, simp)
+   apply(rule_tac \<nu>'="\<lambda>s. 0" and \<mu>'="\<lambda>s. (s$2)^2" in diff_invariant_rules(2); (simp add: forall_2)?)
+  apply(simp add: le_fun_def, rule_tac C="\<lambda>s. s$1 \<ge> 0" in diff_cut_rule, simp_all)
+   apply(subst g_ode_inv_def[symmetric, where I="\<lambda>s. s$1 \<ge> 0"])
+   apply(rule fbox_g_odei, simp add: le_fun_def, simp)
+   apply(rule_tac \<nu>'="\<lambda>s. 0" and \<mu>'="\<lambda>s. (s$2)" in diff_invariant_rules(2); (simp add: forall_2)?)
+  by (simp add: le_fun_def, rule diff_weak_rule, simp add: le_fun_def)
+
+
+subsubsection \<open> Dynamics: Exponential growth (4) \<close> (* sic *)
+
+(* x>0 -> [{x'=x^x}]x>0 *)
+lemma "(\<lambda>s::real^1. s$1 > 0) \<le> |x\<acute>=(\<lambda>s. (\<chi> i. (s$1)\<^sup>2)) & G] (\<lambda>s. s$1 > 0)"
+  apply(subst g_ode_inv_def[symmetric, where I="\<lambda>s. s$1 > 0"])
+   apply(rule fbox_g_odei, simp add: le_fun_def, simp)
+  by (rule_tac \<nu>'="\<lambda>s. 0" and \<mu>'="\<lambda>s. (s$1)\<^sup>2" in diff_invariant_rules(3), simp_all add: le_fun_def)
+
+
+subsubsection \<open> Dynamics: Exponential growth (5) \<close>
+
+(* x>=1 -> [{x'=x\<^sup>2+2*x^4}]x^3>=x\<^sup>2 *)
+lemma "(\<lambda>s::real^1. s$1 \<ge> 1) \<le> 
+  |x\<acute>=(\<lambda>s. (\<chi> i. (s$1)\<^sup>2 + 2 * (s$1)^4)) & G] (\<lambda>s. s$1^3 \<ge> (s$1)\<^sup>2)"
+  apply(rule_tac C="\<lambda>s. s$1 \<ge> 1" in diff_cut_rule; simp?)
+   apply (rule_tac \<nu>'="\<lambda>s. 0" and \<mu>'="\<lambda>s. (s$1)\<^sup>2 + 2 * s$1 ^ 4" in diff_invariant_rules(2); simp?)
+  apply(force intro!: poly_derivatives)
+  apply(subst g_ode_inv_def[symmetric, where I="\<lambda>s. s$1^3 \<ge>  (s$1)\<^sup>2 "])
+apply(rule fbox_g_odei, simp add: le_fun_def, simp_all add: power_increasing)
+  apply (rule_tac \<nu>'="\<lambda>s. 2 * s$1 * ((s$1)\<^sup>2 + 2 * (s$1)^ 4)"
+              and \<mu>'="\<lambda>s. 3 * (s$1)\<^sup>2 * ((s$1)\<^sup>2 + 2 * (s$1)^4)" in diff_invariant_rules(2); clarsimp?)
+  apply(auto intro!: poly_derivatives simp: field_simps semiring_normalization_rules(27,28))
+  apply(subgoal_tac "X \<tau> $ 1 \<ge> 1")
+   apply(subgoal_tac "2 + 4 * (X \<tau>)$1 ^ 2 \<le> 3 * (X \<tau>)$1 + 6 * (X \<tau>)$1 ^ 3")
+    apply (smt One_nat_def numerals(1) one_le_power power.simps(2) power_0 power_add_numeral 
+      power_less_power_Suc power_one_right semiring_norm(2) semiring_norm(4) semiring_norm(5))
+   apply (smt numeral_One one_le_power power_add_numeral power_commutes power_le_one 
+      power_less_power_Suc power_one_right semiring_norm(5))
+  by simp
+
+
+subsubsection \<open> Dynamics: Rotational dynamics (1) \<close>
+
+(* x\<^sup>2+y\<^sup>2=1 -> [{x'=-y, y'=x}]x\<^sup>2+y\<^sup>2=1 *)
+lemma "(\<lambda>s::real^2. (s$1)\<^sup>2 + (s$2)\<^sup>2 = 1) \<le> |x\<acute>= (\<lambda>s.(\<chi> i. if i = 1 then - s$2 else s$1)) & G]
+  (\<lambda>s. (s$1)\<^sup>2 + (s$2)\<^sup>2 = 1)"
+  by (auto intro!: poly_derivatives diff_invariant_rules)
+
+
+subsubsection \<open> Dynamics: Rotational dynamics (2) \<close> (* proved as a linear system *)
+
+(* x\<^sup>2+y\<^sup>2=1 & e=x -> [{x'=-y, y'=e, e'=-y}](x\<^sup>2+y\<^sup>2=1 & e=x) *)
+
+
+subsubsection \<open> Dynamics: Rotational dynamics (3) \<close>
+
+(* d1\<^sup>2+d2\<^sup>2=w\<^sup>2*p\<^sup>2 & d1=-w*x2 & d2=w*x1 -> 
+  [{x1'=d1, x2'=d2, d1'=-w*d2, d2'=w*d1}](d1\<^sup>2+d2\<^sup>2=w\<^sup>2*p\<^sup>2 & d1=-w*x2 & d2=w*x1)*)
+lemma "(\<lambda>s::real^4. (s$3)\<^sup>2 + (s$4)\<^sup>2 = w\<^sup>2 * p\<^sup>2 \<and> s$3 = - w * s$2 \<and> s$4 = w * s$1) \<le> 
+  |x\<acute>= (\<lambda>s. (\<chi> i. if i=1 then s$3 else (if i=2 then s$4 else (if i = 3 then - w * s$4 else w * s$3)))) & G]
+  (\<lambda>s. (s$3)\<^sup>2 + (s$4)\<^sup>2 = w\<^sup>2*p\<^sup>2 \<and> s$3 = - w * s$2 \<and> s$4= w * s$1)"
+  by (auto intro!: diff_invariant_rules poly_derivatives)
+
+
+subsubsection \<open> Dynamics: Spiral to equilibrium \<close>
+
+(* w>=0 & x=0 & y=3 -> [{x'=y, y'=-w\<^sup>2*x-2*w*y}]w\<^sup>2*x\<^sup>2+y\<^sup>2<=9 *)
+lemma "(\<lambda>s::real^3. (s$3) \<ge> 0 \<and> s$1=0 \<and> s$2=3) \<le> 
+  |x\<acute>= (\<lambda>s. (\<chi> i. if i=1 then s$2 else (if i=2 then - (s$3)\<^sup>2*(s$1) - 2*(s$3)*(s$2) else 0))) & G] 
+  (\<lambda>s. (s$3)\<^sup>2*(s$1)\<^sup>2 + (s$2)\<^sup>2 \<le> 9)"
+  apply(rule_tac C="\<lambda>s. s$3 \<ge> 0" in diff_cut_rule; simp?)
+   apply(subst g_ode_inv_def[symmetric, where I="\<lambda>s. s$3 \<ge> 0"])
+   apply(rule fbox_g_odei, simp add: le_fun_def, simp)
+    apply (rule_tac \<nu>'="\<lambda>s. 0" and \<mu>'="\<lambda>s. 0" in diff_invariant_rules(2))
+       apply(simp_all add: forall_3, simp add: le_fun_def)
+  apply(subst g_ode_inv_def[symmetric, where I="\<lambda>s. (s$3)\<^sup>2*(s$1)\<^sup>2 + (s$2)\<^sup>2 \<le> 9"])
+  apply(rule fbox_g_odei, simp add: le_fun_def, simp_all add: power_increasing)
+   apply(rule_tac \<nu>'="\<lambda>s. 2 * (s$3)\<^sup>2 * (s$1) * (s$2) + 2 * (s$2) * (- (s$3)\<^sup>2*(s$1) - 2*(s$3)*(s$2))"
+      and \<mu>'="\<lambda>s. 0" in diff_invariant_rules(2))
+  by (auto intro!: poly_derivatives simp: forall_3 field_simps) 
+    (simp add: mult.assoc[symmetric] power2_eq_square)
+
+
+subsubsection \<open> Dynamics: Open cases \<close>
+
+lemma has_vderiv_mono_test:
+  assumes T_hyp: "is_interval T" 
+    and d_hyp: "D f = f' on T"
+    and xy_hyp: "x\<in>T" "y\<in>T" "x \<le> y" 
+  shows "\<forall>x\<in>T. (0::real) \<le> f' x \<Longrightarrow> f x \<le> f y"
+    and "\<forall>x\<in>T. f' x \<le> 0 \<Longrightarrow> f x \<ge> f y"
+proof-
+  have "{x..y} \<subseteq> T"
+    using T_hyp xy_hyp by (meson atLeastAtMost_iff mem_is_interval_1_I subsetI) 
+  hence "D f = f' on {x..y}"
+    using has_vderiv_on_subset[OF d_hyp(1)] by blast
+  hence "(\<And>t. x \<le> t \<Longrightarrow> t \<le> y \<Longrightarrow> D f \<mapsto> (\<lambda>\<tau>. \<tau> *\<^sub>R f' t) at t within {x..y})"
+    unfolding has_vderiv_on_def has_vector_derivative_def by auto
+  then obtain c where c_hyp: "c \<in> {x..y} \<and> f y - f x = (y - x) *\<^sub>R f' c"
+    using mvt_very_simple[OF xy_hyp(3), of f "(\<lambda>t \<tau>. \<tau> *\<^sub>R f' t)"] by blast
+  hence mvt_hyp: "f x = f y - f' c * (y - x)"
+    by (simp add: mult.commute)
+  also have "\<forall>x\<in>T. 0 \<le> f' x \<Longrightarrow> ... \<le> f y"
+    using xy_hyp d_hyp c_hyp \<open>{x..y} \<subseteq> T\<close> by auto
+  finally show "\<forall>x\<in>T. 0 \<le> f' x \<Longrightarrow> f x \<le> f y" .
+  have "\<forall>x\<in>T. f' x \<le> 0 \<Longrightarrow> f y - f' c * (y - x) \<ge> f y"
+    using xy_hyp d_hyp c_hyp \<open>{x..y} \<subseteq> T\<close> by (auto simp: mult_le_0_iff)
+  thus "\<forall>x\<in>T. f' x \<le> 0 \<Longrightarrow> f x \<ge> f y"
+    using mvt_hyp by auto
+qed
+
+lemma continuous_on_ge_ball_ge: 
+  "continuous_on T f \<Longrightarrow> x \<in> T \<Longrightarrow> f x > (k::real) \<Longrightarrow> \<exists>\<epsilon>>0. \<forall>y\<in>ball x \<epsilon> \<inter> T. f y > k"
+  unfolding continuous_on_iff apply(erule_tac x=x in ballE; clarsimp?)
+  apply(erule_tac x="f x - k" in allE, clarsimp simp: dist_norm)
+  apply(rename_tac \<delta>, rule_tac x=\<delta> in exI, clarsimp)
+  apply(erule_tac x=y in ballE; clarsimp?)
+  by (subst (asm) abs_le_eq, simp_all add: dist_commute)
+
+lemma current_vderiv_ge_always_ge:
+  fixes c::real
+  assumes init: "c < x t\<^sub>0" and ode: "D x = x' on {t\<^sub>0..}" 
+    and dhyp: "x' = (\<lambda>t. g (x t))" "\<forall>x\<ge>c. g x \<ge> 0"
+  shows "\<forall>t\<ge>t\<^sub>0. x t > c"
+proof-
+  have cont: "continuous_on {t\<^sub>0..} x"
+    using vderiv_on_continuous_on[OF ode] .
+  {assume "\<exists>t\<ge>t\<^sub>0. x t \<le> c"
+    hence inf: "{t. t > t\<^sub>0 \<and> x t \<le> c} \<noteq> {}" "bdd_below {t. t > t\<^sub>0 \<and> x t \<le> c}"
+      using init less_eq_real_def unfolding bdd_below_def by force (rule_tac x=t\<^sub>0 in exI, simp)
+    define t\<^sub>1 where t1_hyp: "t\<^sub>1 = Inf {t. t > t\<^sub>0 \<and> x t \<le> c}"
+    hence "t\<^sub>0 \<le> t\<^sub>1"  
+      using le_cInf_iff[OF inf, of t\<^sub>0] by auto
+    have "x t\<^sub>1 \<ge> c"
+    proof-
+      {assume "x t\<^sub>1 < c"
+        hence obs: "x t\<^sub>1 \<le> c" "x t\<^sub>0 \<ge> c" "t\<^sub>1 \<noteq> t\<^sub>0"
+          using init by auto
+        hence "t\<^sub>1 > t\<^sub>0"
+          using \<open>t\<^sub>0 \<le> t\<^sub>1\<close> by auto
+        then obtain k where k2_hyp: "k \<ge> t\<^sub>0 \<and> k \<le> t\<^sub>1 \<and> x k = c"
+          using IVT2'[of "\<lambda>t. x t", OF obs(1,2) _ continuous_on_subset[OF cont]] by auto
+        hence "t\<^sub>0 < k" "k < t\<^sub>1"
+          using \<open>x t\<^sub>1 < c\<close> less_eq_real_def init by auto
+        also have "t\<^sub>1 \<le> k"
+          using cInf_lower[OF _ inf(2)] k2_hyp calculation unfolding t1_hyp by auto
+        ultimately have False
+          by simp}
+      thus "x t\<^sub>1 \<ge> c"
+        by fastforce
+    qed
+    hence obs: "\<forall>t\<in>{t\<^sub>0..<t\<^sub>1}. x t > c"
+    proof-
+      {assume "\<exists>t\<in>{t\<^sub>0..<t\<^sub>1}. x t \<le> c"
+        then obtain k where k2_hyp: "k \<ge> t\<^sub>0 \<and> k < t\<^sub>1 \<and> x k \<le> c"
+          by auto
+        hence "k > t\<^sub>0"
+          using \<open>x t\<^sub>0 > c\<close> less_eq_real_def by auto
+        hence "t\<^sub>1 \<le> k"
+          using cInf_lower[OF _ inf(2)] k2_hyp unfolding t1_hyp by auto
+        hence "False"
+          using k2_hyp by auto}
+      thus "\<forall>t\<in>{t\<^sub>0..<t\<^sub>1}. x t > c"
+        by force
+    qed
+    hence "\<forall>t\<in>{t\<^sub>0..t\<^sub>1}. x' t \<ge> 0"
+      using \<open>x t\<^sub>1 \<ge> c\<close> dhyp(2) less_eq_real_def 
+      unfolding dhyp by (metis atLeastAtMost_iff atLeastLessThan_iff) 
+    hence "x t\<^sub>0 \<le> x t\<^sub>1"
+      apply(rule_tac f="\<lambda>t. x t" and T="{t\<^sub>0..t\<^sub>1}" in has_vderiv_mono_test(1); clarsimp)
+      using has_vderiv_on_subset[OF ode] apply force
+      using \<open>t\<^sub>0  \<le> t\<^sub>1\<close>  by (auto simp: less_eq_real_def)
+    hence "c < x t\<^sub>1"
+      using \<open>x t\<^sub>1 \<ge> c\<close> init by auto
+    then obtain \<epsilon> where eps_hyp: "\<epsilon> > 0 \<and> (\<forall>t\<in>ball t\<^sub>1 \<epsilon> \<inter> {t\<^sub>0..}. c < x t)"
+      using continuous_on_ge_ball_ge[of _ "\<lambda>t. x t", OF cont _ \<open>c < x t\<^sub>1\<close>] \<open>t\<^sub>0  \<le> t\<^sub>1\<close> by auto
+    hence "\<forall>t\<in>{t\<^sub>0..<t\<^sub>1+\<epsilon>}. c < x t"
+      using obs \<open>t\<^sub>0 \<le> t\<^sub>1\<close> ball_eq_greaterThanLessThan by auto
+    hence "\<forall>t\<in>{t. t > t\<^sub>0 \<and> x t \<le> c}. t\<^sub>1+\<epsilon> \<le> t"
+      by (metis (mono_tags, lifting) atLeastLessThan_iff less_eq_real_def mem_Collect_eq not_le)
+    hence "t\<^sub>1+\<epsilon> \<le> t\<^sub>1"
+      using le_cInf_iff[OF inf] unfolding t1_hyp by simp
+    hence False
+      using eps_hyp by auto}
+  thus "\<forall>t\<ge>t\<^sub>0. c < x t"
+    by fastforce
+qed
+
+(* x^3>5 & y>2 -> [{x'=x^3+x^4, y'=5*y+y^2}](x^3>5 & y>2) *)
+lemma "0 \<le> t \<Longrightarrow> (\<lambda>s::real^2. s$1^3>5 \<and> s$2>2) \<le> 
+  |x\<acute>= (\<lambda>t s. (\<chi> i. if i=1 then s$1^3 + s$1^4 else 5 * s$2 + s$2^2)) & G on (\<lambda>s. {0..}) UNIV @ 0]
+  (\<lambda>s. s$1^3>5 \<and> s$2>2)"
+  apply(simp, rule diff_invariant_rules, simp_all add: diff_invariant_eq ivp_sols_def forall_2; clarsimp)
+   apply(frule_tac x="\<lambda>t. X t $ 1 ^ 3" and g="\<lambda>t. 3 * t^2 + 3 * (root 3 t)^5" in current_vderiv_ge_always_ge)
+      apply(rule poly_derivatives, simp, assumption, simp)
+     apply (force simp: field_simps odd_real_root_power_cancel, force simp: add_nonneg_pos, force)
+  apply(frule_tac x="\<lambda>t. X t $ 2" in current_vderiv_ge_always_ge)
+  by (force, force, force simp: add_nonneg_pos, simp)
+
+
+subsubsection \<open> Dynamics: Closed cases \<close>
+
+(* x>=1 & y=10 & z=-2 -> [{x'=y, y'=z+y^2-y & y>=0}](x>=1 & y>=0) *)
+lemma "z = - 2 \<Longrightarrow> (\<lambda>s::real^2. s$1 \<ge> 1 \<and> s$2 = 10) \<le> 
+  |x\<acute>= (\<lambda>s. (\<chi> i. if i=1 then s$2 else z + (s$2)^2 - s$2)) & (\<lambda>s. s$2 \<ge> 0)]
+  (\<lambda>s. s$1 \<ge> 1 \<and> s$2 \<ge> 0)"
+  apply(subst g_ode_inv_def[symmetric, where I="\<lambda>s. s$1 \<ge> 1 \<and> s$2 \<ge> 0"])
+  apply(rule fbox_g_odei, simp_all, simp add: le_fun_def, rule diff_invariant_rules)
+   apply(rule_tac \<nu>'="\<lambda>s. 0" and \<mu>'="\<lambda>s. s$2" in diff_invariant_rules(2))
+  by (simp_all add: diff_invariant_eq, force intro!: poly_derivatives)
+
+
+subsubsection \<open> Dynamics: Conserved quantity \<close>
+
+lemma dyn_cons_qty_arith: "(36::real) * (x1\<^sup>2 * (x1 * x2 ^ 3)) - 
+  (- (24 * (x1\<^sup>2 * x2) * x1 ^ 3 * (x2)\<^sup>2) - 12 * (x1\<^sup>2 * x2) * x1 * x2 ^ 4) - 
+  36 * (x1\<^sup>2 * (x2 * x1)) * (x2)\<^sup>2 - 12 * (x1\<^sup>2 * (x1 * x2 ^ 5)) = 24 * (x1 ^ 5 * x2 ^ 3)" 
+  (is "?t1 - (- ?t2 - ?t3) - ?t4 - ?t5 = ?t6")
+proof-
+  have eq1: "?t1 = ?t4"
+    by (simp add: power2_eq_square power3_eq_cube)
+  have eq2: "- (- ?t2 - ?t3) = (?t6 + ?t3)"
+    by (auto simp: field_simps semiring_normalization_rules(27))
+  have eq3: "?t3 = ?t5"
+    by (auto simp: field_simps semiring_normalization_rules(27))
+  show "?t1 - (- ?t2 - ?t3) - ?t4 - ?t5 = ?t6"
+    unfolding eq1 eq2 eq3 by (simp add: field_simps semiring_normalization_rules(27))
+qed
+
+(* x1^4*x2^2+x1^2*x2^4-3*x1^2*x2^2+1 <= c ->
+    [{x1'=2*x1^4*x2+4*x1^2*x2^3-6*x1^2*x2, x2'=-4*x1^3*x2^2-2*x1*x2^4+6*x1*x2^2}] 
+   x1^4*x2^2+x1^2*x2^4-3*x1^2*x2^2+1 <= c *)
+lemma "(\<lambda>s::real^2. (s$1)^4*(s$2)^2+(s$1)^2*(s$2)^4-3*(s$1)^2*(s$2)^2 + 1 \<le> c) \<le> 
+  |x\<acute>= (\<lambda>s. (\<chi> i. if i=1 then 2*(s$1)^4*(s$2)+4*(s$1)^2*(s$2)^3-6*(s$1)^2*(s$2) 
+    else -4*(s$1)^3*(s$2)^2-2*(s$1)*(s$2)^4+6*(s$1)*(s$2)^2)) & G] 
+  (\<lambda>s. (s$1)^4*(s$2)^2+(s$1)^2*(s$2)^4-3*(s$1)^2*(s$2)^2 + 1 \<le> c)"
+  apply(simp, rule_tac \<mu>'="\<lambda>s. 0" and \<nu>'="\<lambda>s. 0" in diff_invariant_rules(2); clarsimp simp: forall_2)
+  apply(intro poly_derivatives; (assumption)?, (rule poly_derivatives)?)
+  apply force+
+  apply(clarsimp simp: algebra_simps(17,18,19,20) semiring_normalization_rules(27,28))
+  by (auto simp: dyn_cons_qty_arith)
+
+
+subsubsection \<open> Dynamics: Darboux equality \<close>
+
+lemma mult_abs_right_mono: "a < b \<Longrightarrow> a * \<bar>c\<bar> \<le> b * \<bar>c\<bar>" for c::real
+  by (simp add: mult_right_mono)
+
+lemma local_lipschitz_first_order_linear:
+  fixes c::"real \<Rightarrow> real"
+  assumes "continuous_on T c"
+  shows "local_lipschitz T UNIV (\<lambda>t. (*) (c t))"
+proof(unfold local_lipschitz_def lipschitz_on_def, clarsimp simp: dist_norm)
+  fix x t::real assume "t \<in> T"
+  then obtain \<delta> where d_hyp: "\<delta> > 0 \<and> (\<forall>\<tau>\<in>T. \<bar>\<tau> - t\<bar> < \<delta> \<longrightarrow> \<bar>c \<tau> - c t\<bar> < max 1 \<bar>c t\<bar>)"
+    using assms unfolding continuous_on_iff 
+    apply(erule_tac x=t in ballE, erule_tac x="max 1 (\<bar>c t\<bar>)" in allE; clarsimp)
+    by (metis dist_norm less_max_iff_disj real_norm_def zero_less_one)
+  {fix \<tau> x\<^sub>1 x\<^sub>2 
+    assume "\<tau> \<in> cball t (\<delta>/2) \<inter> T" "x\<^sub>1 \<in> cball x (\<delta>/2)" "x\<^sub>2 \<in> cball x (\<delta>/2)" 
+    hence "\<bar>\<tau> - t\<bar> < \<delta>" "\<tau> \<in> T"
+      by (auto simp: dist_norm, smt d_hyp)
+    hence "\<bar>c \<tau> - c t\<bar> < max 1 \<bar>c t\<bar>"
+      using d_hyp by auto
+    hence "- (max 1 \<bar>c t\<bar> + \<bar>c t\<bar>) < c \<tau> \<and> c \<tau> < max 1 \<bar>c t\<bar> + \<bar>c t\<bar>"
+      by (auto simp: abs_le_eq)
+    hence obs: "\<bar>c \<tau>\<bar> < max 1 \<bar>c t\<bar> + \<bar>c t\<bar>"
+      by (simp add: abs_le_eq)
+    have "\<bar>c \<tau> * x\<^sub>1 - c \<tau> * x\<^sub>2\<bar> = \<bar>c \<tau>\<bar> * \<bar>x\<^sub>1 - x\<^sub>2\<bar>"
+      by (metis abs_mult left_diff_distrib mult.commute)
+    also have "... \<le> (max 1 \<bar>c t\<bar> + \<bar>c t\<bar>) * \<bar>x\<^sub>1 - x\<^sub>2\<bar>"
+      using mult_abs_right_mono[OF obs] by blast
+    finally have "\<bar>c \<tau> * x\<^sub>1 - c \<tau> * x\<^sub>2\<bar> \<le> (max 1 \<bar>c t\<bar> + \<bar>c t\<bar>) * \<bar>x\<^sub>1 - x\<^sub>2\<bar>" .}
+  hence "\<exists>L. \<forall>t\<in>cball t (\<delta>/2) \<inter> T. 0 \<le> L \<and>
+    (\<forall>x\<^sub>1\<in>cball x (\<delta>/2). \<forall>x\<^sub>2\<in>cball x (\<delta>/2). \<bar>c t * x\<^sub>1 - c t * x\<^sub>2\<bar> \<le> L * \<bar>x\<^sub>1 - x\<^sub>2\<bar>)"
+    by (rule_tac x="max 1 \<bar>c t\<bar> + \<bar>c t\<bar>" in exI, clarsimp simp: dist_norm)
+  thus "\<exists>u>0. \<exists>L. \<forall>t\<in>cball t u \<inter> T. 0 \<le> L \<and> 
+    (\<forall>xa\<in>cball x u. \<forall>y\<in>cball x u. \<bar>c t * xa - c t * y\<bar> \<le> L * \<bar>xa - y\<bar>)"
+    apply(rule_tac x="\<delta>/2" in exI) 
+    using d_hyp by auto
+qed
+
+lemma picard_lindeloef_first_order_linear: "t\<^sub>0 \<in> T \<Longrightarrow> open T \<Longrightarrow> is_interval T \<Longrightarrow> 
+  continuous_on T c \<Longrightarrow> picard_lindeloef (\<lambda>t x::real. c t * x) T UNIV t\<^sub>0"
+  apply(unfold_locales; clarsimp?)
+   apply(intro continuous_intros, assumption)
+  by (rule local_lipschitz_first_order_linear)
+
+(* x+z=0 -> [{x'=(A*x^2+B()*x), z' = A*z*x+B()*z}] 0=-x-z *)
+lemma "(\<lambda>s::real^2. s$1 + s$2 = 0) \<le> 
+  |x\<acute>= (\<lambda>t s. (\<chi> i. if i=1 then A*(s$1)^2+B*(s$1) else A*(s$2)*(s$1)+B*(s$2))) & G on (\<lambda>s. UNIV) UNIV @ 0]
+  (\<lambda>s. 0 = - s$1 - s$2)"
+proof-
+  have key: "diff_invariant (\<lambda>s. s $ 1 + s $ 2 = 0)
+     (\<lambda>t s. \<chi> i. if i = 1 then A*(s$1)^2+B*(s$1) else A*(s$2)*(s$1)+B*(s$2)) (\<lambda>s. UNIV) UNIV 0 G"
+  proof(clarsimp simp: diff_invariant_eq ivp_sols_def forall_2)
+    fix X::"real\<Rightarrow>real^2" and t::real
+    let "?c" = "(\<lambda>t.  X t $ 1 + X t $ 2)"
+    assume init: "?c 0 = 0"
+      and D1: "D (\<lambda>t. X t $ 1) = (\<lambda>t. A * (X t $ 1)\<^sup>2 + B * X t $ 1) on UNIV"
+      and D2: "D (\<lambda>t. X t $ 2) = (\<lambda>t. A * X t $ 2 * X t $ 1 + B * X t $ 2) on UNIV"
+    hence "D ?c = (\<lambda>t. ?c t * (A * (X t $ 1) + B)) on UNIV"
+      by (auto intro!: poly_derivatives simp: field_simps power2_eq_square)
+    hence "D ?c = (\<lambda>t. (A * X t $ 1 + B) * (X t $ 1 + X t $ 2)) on {0--t}"
+      using has_vderiv_on_subset[OF _ subset_UNIV[of "{0--t}"]] by (simp add: mult.commute)
+    moreover have "continuous_on UNIV (\<lambda>t. A * (X t $ 1) + B)"
+      apply(rule vderiv_on_continuous_on)
+      using D1 by (auto intro!: poly_derivatives simp: field_simps power2_eq_square)
+    moreover have "D (\<lambda>t. 0) = (\<lambda>t. (A * X t $ 1 + B) * 0) on {0--t}"
+      by (auto intro!: poly_derivatives)
+    moreover note picard_lindeloef.ivp_unique_solution[OF 
+      picard_lindeloef_first_order_linear[OF UNIV_I open_UNIV is_interval_univ calculation(2)] 
+      UNIV_I is_interval_closed_segment_1 subset_UNIV _ 
+      ivp_solsI[of ?c]
+      ivp_solsI[of "\<lambda>t. 0"], of t "\<lambda>s. 0" 0 "\<lambda>s. t" 0]
+    ultimately show "X t $ 1 + X t $ 2 = 0"
+      using init by auto
+  qed
+  show ?thesis
+    apply(subgoal_tac "(\<lambda>s. 0 = - s$1 - s$2) = (\<lambda>s. s$1 + s$2 = 0)", erule ssubst)
+    using key by auto
+qed
+
+
+subsubsection \<open> Dynamics: Fractional Darboux equality \<close> (*N 30 *)
+
+(* x+z=0 -> [{x'=(A*y+B()*x)/z^2, z' = (A*x+B())/z & y = x^2 & z^2 > 0}] x+z=0 *)
+(* requires picard-lindeloef for closed intervals *)
+
+subsubsection \<open> Dynamics: Darboux inequality \<close> (*N 31 *)
+
+abbreviation darboux_ineq_f :: "real^2 \<Rightarrow> real^2" ("f")
+  where "f s \<equiv> (\<chi> i. if i=1 then (s$1)^2 else (s$2)*(s$1)+(s$1)^2)"
+
+abbreviation darboux_ineq_flow2 :: "real \<Rightarrow> real^2 \<Rightarrow> real^2" ("\<phi>")
+  where "\<phi> t s \<equiv> (\<chi> i. if i=1 then (s$1/(1 - t * s$1)) else
+      (s$2 - s$1 * ln(1 - t * s$1))/(1 - t * s$1))"
+
+lemma darboux_flow_ivp: "(\<lambda>t. \<phi> t s) \<in> Sols (\<lambda>t. f) (\<lambda>s. {t. 0 \<le> t \<and> t * s $ 1 < 1}) UNIV 0 s"
+  by (rule ivp_solsI) (auto intro!: poly_derivatives 
+      simp: forall_2 power2_eq_square add_divide_distrib power_divide vec_eq_iff)
+
+lemma darboux_ineq_arith:
+  assumes "0 \<le> s\<^sub>1 + s\<^sub>2" and "0 \<le> (t::real)" and "t * s\<^sub>1 < 1"
+  shows "0 \<le> s\<^sub>1 / (1 - t * s\<^sub>1) + (s\<^sub>2 - s\<^sub>1 * ln (1 - t * s\<^sub>1)) / (1 - t * s\<^sub>1)"
+proof-
+  have "s\<^sub>1 * ln (1 - t * s\<^sub>1) \<le> 0"
+  proof(cases "s\<^sub>1 \<le> 0")
+    case True
+    hence "1 - t * s\<^sub>1 \<ge> 1"
+      using \<open>0 \<le> t\<close> by (simp add: mult_le_0_iff)
+    thus ?thesis
+      using True ln_ge_zero mult_nonneg_nonpos2 by blast
+  next
+    case False
+    hence "1 - t * s\<^sub>1 \<le> 1"
+      using \<open>0 \<le> t\<close> by auto
+    thus ?thesis
+      by (metis (mono_tags, hide_lams) False add.left_neutral antisym_conv assms(3) 
+          diff_le_eq ln_ge_zero_iff ln_one mult_zero_right not_le order_refl zero_le_mult_iff)
+  qed
+  hence "s\<^sub>1 + s\<^sub>2 - s\<^sub>1 * ln (1 - t * s\<^sub>1) \<ge> s\<^sub>1 + s\<^sub>2"
+    by linarith
+  hence "(s\<^sub>1 + s\<^sub>2 - s\<^sub>1 * ln (1 - t * s\<^sub>1))/(1 - t * s\<^sub>1) \<ge> (s\<^sub>1 + s\<^sub>2)/(1 - t * s\<^sub>1)"
+    using \<open>t * s\<^sub>1 < 1\<close> by (simp add: \<open>0 \<le> s\<^sub>1 + s\<^sub>2\<close> divide_right_mono)
+  also have "(s\<^sub>1 + s\<^sub>2)/(1 - t * s\<^sub>1) \<ge> 0"
+    using \<open>t * s\<^sub>1 < 1\<close> by (simp add: \<open>0 \<le> s\<^sub>1 + s\<^sub>2\<close>)
+  ultimately show ?thesis
+    by (metis (full_types) add_diff_eq add_divide_distrib order_trans)
+qed
+
+(* x+z>=0 -> [{x'=x^2, z' = z*x+y & y = x^2}] x+z>=0 *)
+(* x' + z' \<ge> 0 \<longleftrightarrow> x^2 + z*x + x^2 \<ge> 0*)
+lemma "(\<lambda>s::real^2. s$1 + s$2 \<ge> 0) \<le> 
+  |EVOL \<phi> (\<lambda>s. y = (s$1)^2) (\<lambda>s. {t. 0 \<le> t \<and> t * s $ 1 < 1})]
+  (\<lambda>s. s$1 + s$2 \<ge> 0)"
+  apply(subst fbox_g_evol, simp_all add: le_fun_def)
+  using darboux_ineq_arith by smt
+
+no_notation darboux_ineq_flow2 ("\<phi>")
+        and darboux_ineq_f ("f")
+
+(* interval of existence or invariant rule for \<le> *)
+
+
+subsubsection \<open> Dynamics: Bifurcation \<close>
+
+lemma picard_lindeloef_dyn_bif: "continuous_on T (g::real \<Rightarrow> real) \<Longrightarrow> t\<^sub>0 \<in> T \<Longrightarrow> is_interval T \<Longrightarrow> 
+  open T \<Longrightarrow> picard_lindeloef (\<lambda>t \<tau>::real. r + \<tau>^2) T UNIV t\<^sub>0"
+proof(unfold_locales; clarsimp simp: dist_norm local_lipschitz_def lipschitz_on_def)
+  fix x t::real
+  {fix x1 and x2
+    assume "x1 \<in>cball x 1" and "x2 \<in>cball x 1"
+    hence leq: "\<bar>x - x1\<bar> \<le> 1" "\<bar>x - x2\<bar> \<le> 1"
+      by (auto simp: dist_norm)
+    have "\<bar>x1 + x2\<bar> = \<bar>x1 - x + x2 - x + 2 * x\<bar>"
+      by simp
+    also have "... \<le> \<bar>x1 - x\<bar> + \<bar>x2 - x\<bar> + 2 * \<bar>x\<bar>"
+      using abs_triangle_ineq by auto
+    also have "... \<le> 2 * (1 + \<bar>x\<bar>)"
+      using leq by auto
+    finally have obs: "\<bar>x1 + x2\<bar> \<le> 2 * (1 + \<bar>x\<bar>)" .
+    also have "\<bar>x1\<^sup>2 - x2\<^sup>2\<bar> = \<bar>x1 + x2\<bar>*\<bar>x1 - x2\<bar>"
+      by (metis abs_mult power2_eq_square square_diff_square_factored)
+    ultimately have "\<bar>x1\<^sup>2 - x2\<^sup>2\<bar> \<le> (2 * (1 + \<bar>x\<bar>)) * \<bar>x1 - x2\<bar>"
+      by (metis abs_ge_zero mult_right_mono)}
+  thus "\<exists>u>0. (\<exists>\<tau>. \<bar>t - \<tau>\<bar> \<le> u \<and> \<tau> \<in> T) \<longrightarrow> 
+  (\<exists>L\<ge>0. \<forall>xa\<in>cball x u. \<forall>y\<in>cball x u. \<bar>xa\<^sup>2 - y\<^sup>2\<bar> \<le> L * \<bar>xa - y\<bar>)"
+    by (rule_tac x=1 in exI, clarsimp, rule_tac x="2 * (1 + \<bar>x\<bar>)" in exI, auto)
+qed
+
+(* r <= 0 -> \exists f (x=f -> [{x'=r+x^2}]x=f) *)
+lemma "r \<le> 0 \<Longrightarrow> \<exists>c. (\<lambda>s::real^1. s$1 = c) \<le> 
+  |x\<acute>= (\<lambda>t s. (\<chi> i. r + (s$1)^2)) & G on (\<lambda>s. UNIV) UNIV @ 0] 
+  (\<lambda>s. s$1 = c)"
+proof(rule_tac x="sqrt \<bar>r\<bar>" in exI, clarsimp simp: diff_invariant_eq ivp_sols_def)
+  fix X::"real\<Rightarrow>real^1" and t::real
+  assume init: "X 0 $ 1 = sqrt (- r)" and "r \<le> 0"
+     and D1: "D (\<lambda>x. X x $ 1) = (\<lambda>x. r + (X x $ 1)\<^sup>2) on UNIV"
+  hence "D (\<lambda>x. X x $ 1) = (\<lambda>x. r + (X x $ 1)\<^sup>2) on {0--t}"
+    using has_vderiv_on_subset by blast
+  moreover have "continuous_on UNIV (\<lambda>t. X t $ 1)"
+    apply(rule vderiv_on_continuous_on)
+    using D1 by assumption
+  moreover have key: "D (\<lambda>t. sqrt (- r)) = (\<lambda>t. r + (sqrt (- r))\<^sup>2) on {0--t}"
+    apply(subgoal_tac "(\<lambda>t. r + (sqrt (- r))\<^sup>2) = (\<lambda>t. 0)")
+     apply(erule ssubst, rule poly_derivatives)
+    using \<open>r \<le> 0\<close> by auto
+  moreover note picard_lindeloef.ivp_unique_solution[OF 
+      picard_lindeloef_dyn_bif[OF calculation(2) UNIV_I is_interval_univ open_UNIV] 
+      UNIV_I is_interval_closed_segment_1 subset_UNIV _ 
+      ivp_solsI[of "\<lambda>x. X x $ 1" _ "\<lambda>s. {0--t}" "sqrt (- r)" 0]
+      ivp_solsI[of "\<lambda>t. sqrt (- r)" _], of t r]
+  ultimately show "X t $ 1 = sqrt (- r)"
+    using \<open>r \<le> 0\<close> init by auto
+qed
+
+subsubsection \<open> Dynamics: Parametric switching between two different damped oscillators \<close> (*N 33 *)
+
+(*     w>=0 & d>=0
+  & -2<=a&a<=2
+  & b^2>=1/3
+  & w^2*x^2+y^2 <= c
+->
+  [{
+    {x'=y, y'=-w^2*x-2*d*w*y};
+    {  { ?(x=y*a); w:=2*w; d:=d/2; c := c * ((2*w)^2+1^2) / (w^2+1^2); }
+    ++ { ?(x=y*b); w:=w/2; d:=2*d; c := c * (w^2+1^2) / ((2*w^2)+1^2); }
+    ++ { ?true; } }
+   }*@invariant(w^2*x^2+y^2<=c&d>=0&w>=0)
+  ] w^2*x^2+y^2 <= c *)
+
+(* verified with the help of a CAS *)
+
+
+subsubsection \<open> Dynamics: Nonlinear 1 \<close>
+
+(* x^3 >= -1 -> [{x'=(x-3)^4+a & a>=0}] x^3>=-1 *)
+lemma "(\<lambda>s::real^1. s$1^3 \<ge> -1) \<le> 
+  |x\<acute>= (\<lambda>s. \<chi> i. (s$1 - 3)^4 + a) & (\<lambda>s. a \<ge> 0)]
+  (\<lambda>s. s$1^3 \<ge> -1)"
+  apply(simp, rule_tac \<nu>'="\<lambda>s. 0" and \<mu>'="\<lambda>s. 3 * s$1^2 * ((s$1 - 3)^4 + a)" in diff_invariant_rules(2))
+  by (auto intro!: poly_derivatives simp: field_simps)
+
+
+subsubsection \<open> Dynamics: Nonlinear 2 \<close>
+
+(* x1+x2^2/2=a -> [{x1'=x1*x2,x2'=-x1}]x1+x2^2/2=a *)
+lemma "(\<lambda>s::real^2. s$1 + (s$2^2)/2 = a) \<le> 
+  |x\<acute>= (\<lambda>s. \<chi> i. if i=1 then s$1 * s$2 else - s$1) & G]
+  (\<lambda>s. s$1 + (s$2^2)/2 = a)"
+  by (auto intro!: diff_invariant_rules poly_derivatives)
+
+
+subsubsection \<open> Dynamics: Nonlinear 4 \<close>
+
+(* x1^2/2-x2^2/2>=a -> [{x1'=x2+x1*x2^2, x2'=-x1+x1^2*x2 & x1>=0 & x2>=0}]x1^2/2-x2^2/2>=a *)
+lemma "(\<lambda>s::real^2. (s$1)^2/2 - (s$2^2)/2 \<ge> a) \<le> 
+  |x\<acute>= (\<lambda>s. \<chi> i. if i=1 then s$2 + s$1 * (s$2^2) else - s$1 + s$1^2 * s$2) & (\<lambda>s. s$1 \<ge> 0 \<and> s$2 \<ge> 0)]
+  (\<lambda>s. (s$1)^2/2 - (s$2^2)/2 \<ge> a)"
+  apply(simp, rule_tac \<nu>'="\<lambda>s. 0" and \<mu>'="\<lambda>s. s$1*(s$2 + s$1 * (s$2^2)) - s$2 * (- s$1 + s$1^2 * s$2)" in diff_invariant_rules(2))
+  by (auto intro!: poly_derivatives simp: field_simps power2_eq_square)
+
+
+subsubsection \<open> Dynamics: Nonlinear 5 \<close>
+
+(* -x1*x2>=a -> [{x1'=x1-x2+x1*x2, x2'=-x2-x2^2}]-x1*x2>=a *)
+lemma "(\<lambda>s::real^2. -(s$1) *(s$2) \<ge> a) \<le> 
+  |x\<acute>= (\<lambda>s. \<chi> i. if i=1 then s$1 - s$2 + s$1 * s$2 else - s$2 - s$2^2) & G]
+  (\<lambda>s. -(s$1)*(s$2) \<ge> a)"
+  apply(simp, rule_tac \<nu>'="\<lambda>s. 0" and \<mu>'="\<lambda>s. (- s$1 + s$2 - s$1 * s$2) * s$2 - s$1 * (- s$2 - s$2^2)" in diff_invariant_rules(2))
+  by (auto intro!: poly_derivatives simp: field_simps power2_eq_square)
+
+
+subsubsection \<open> Dynamics: Riccati \<close>
+
+(* 2*x^3 >= 1/4 -> [{x'=x^2+x^4}] 2*x^3>=1/4 *)
+lemma "(\<lambda>s::real^1. 2 * s$1^3 \<ge> 1/4) \<le> 
+  |x\<acute>= (\<lambda>s. \<chi> i. s$1^2 + s$1^4) & G]
+  (\<lambda>s. 2 * s$1^3 \<ge> 1/4)"
+  apply(simp, rule_tac \<nu>'="\<lambda>s. 0" and \<mu>'="\<lambda>s. 24 * (s$1^2) * (s$1^2 + s$1^4)" in diff_invariant_rules(2); clarsimp)
+  by (auto intro!: poly_derivatives simp: field_simps power2_eq_square)
+
+
+subsubsection \<open> Dynamics: Nonlinear differential cut \<close>
+
+(* x^3 >= -1 & y^5 >= 0 -> [{x'=(x-3)^4+y^5, y'=y^2}] (x^3 >= -1 & y^5 >= 0) *)
+lemma "(\<lambda>s::real^2. s$1^3 \<ge> - 1 \<and> s$2^5 \<ge> 0) \<le> 
+  |x\<acute>= (\<lambda>s. \<chi> i. if i=1 then (s$1 - 3)^4 else s$2^2) & G]
+  (\<lambda>s. s$1^3 \<ge> - 1 \<and> s$2^5 \<ge> 0)"
+  apply(simp, rule diff_invariant_rules)
+   apply(rule_tac \<nu>'="\<lambda>s. 0" and \<mu>'="\<lambda>s. 3 * s$1^2 * (s$1 - 3)^4" in diff_invariant_rules(2))
+   apply(simp_all add: forall_2, force intro!: poly_derivatives)
+   apply(rule_tac \<nu>'="\<lambda>s. 0" and \<mu>'="\<lambda>s. s$2^2" in diff_invariant_rules(2))
+  by (auto intro!: diff_invariant_rules poly_derivatives simp: forall_2)
+
+
+subsubsection \<open> STTT Tutorial: Example 1 \<close>
+
+(* v >= 0 & A > 0 -> [ { x' = v, v' = A } ] v >= 0 *)
+lemma "A > 0 \<Longrightarrow> (\<lambda>s::real^2. s$2 \<ge> 0) \<le> 
+  |x\<acute>= (\<lambda>s. \<chi> i. if i=1 then s$2 else A) & G]
+  (\<lambda>s. s$2 \<ge> 0)"
+  apply(subst local_flow.fbox_g_ode_subset[where T="UNIV" 
+        and \<phi>="\<lambda>t s. \<chi> i::2. if i=1 then A * t^2/2 + s$2 * t + s$1 else A * t + s$2"])
+      apply(unfold_locales, simp_all add: local_lipschitz_def forall_2 lipschitz_on_def)
+    apply(clarsimp, rule_tac x=1 in exI)+
+  apply(clarsimp simp: dist_norm norm_vec_def L2_set_def)
+  unfolding UNIV_2 using exhaust_2 by (auto intro!: poly_derivatives simp: vec_eq_iff)
+
+
+subsubsection \<open> STTT Tutorial: Example 2 \<close>
+
+(* v >= 0 & A > 0 & B > 0 -> 
+  [
+    { {a := A; ++ a := 0; ++ a := -B;};
+      { x' = v, v' = a & v >= 0 }
+    }*@invariant(v >= 0)
+  ] v >= 0 *)
+
+lemma local_flow_STTT_Ex2:
+  "local_flow (\<lambda>s::real^3. \<chi> i. if i = 1 then s$2 else (if i=2 then s$3 else 0)) UNIV UNIV
+  (\<lambda>t s. \<chi> i. if i = 1 then s$3 * t^2/2 + s$2 * t + s$1 else (if i=2 then s$3 * t + s$2 else s$i))"
+  apply(unfold_locales, simp_all add: local_lipschitz_def forall_2 lipschitz_on_def)
+    apply(clarsimp, rule_tac x=1 in exI)+
+  apply(clarsimp simp: dist_norm norm_vec_def L2_set_def)
+  unfolding UNIV_3 by (auto intro!: poly_derivatives simp: forall_3 vec_eq_iff)
+
+lemma "A > 0 \<Longrightarrow> B > 0 \<Longrightarrow> (\<lambda>s::real^3. s$2 \<ge> 0) \<le>
+  |LOOP (
+    (\<lambda>s. (3 ::= (\<lambda>s. A)) s \<union> (3 ::= (\<lambda>s. 0)) s \<union> (3 ::= (\<lambda>s. B)) s);
+    (x\<acute>= (\<lambda>s. \<chi> i. if i=1 then s$2 else (if i=2 then s$3 else 0)) & (\<lambda>s. s$2 \<ge> 0))
+  ) INV (\<lambda>s. s$2 \<ge> 0)]
+  (\<lambda>s. s$2 \<ge> 0)"
+  apply(rule fbox_loopI, simp_all add: le_fbox_choice_iff, intro conjI)
+  by (simp_all add: local_flow.fbox_g_ode_subset[OF local_flow_STTT_Ex2], simp_all add: le_fun_def)
+
+
+subsubsection \<open> STTT Tutorial: Example 3a \<close> (* 37 *)
+
+(* v >= 0 & A > 0 & B > 0 & x+v^2/(2*B) < S
+ -> [
+      { {   ?x+v^2/(2*B) < S; a := A;
+         ++ ?v=0; a := 0;
+         ++ a := -B;
+        }
+
+        {
+           {x' = v, v' = a & v >= 0 & x+v^2/(2*B) <= S}
+        ++ {x' = v, v' = a & v >= 0 & x+v^2/(2*B) >= S}
+        }
+      }*@invariant(v >= 0 & x+v^2/(2*B) <= S)
+    ] x <= S *)
+
+lemma STTexample3a_arith:
+  assumes "0 < (B::real)" "0 \<le> t" "0 \<le> x2" and key: "x1 + x2\<^sup>2 / (2 * B) \<le> S"
+  shows "x2 * t - B * t\<^sup>2 / 2 + x1 + (x2 - B * t)\<^sup>2 / (2 * B) \<le> S" (is "?lhs \<le> S")
+proof-
+  have "?lhs = 2 * B * x2 * t/(2*B) - B^2 * t\<^sup>2 / (2*B) + (2 * B * x1)/(2*B) + (x2 - B * t)\<^sup>2 / (2 * B)"
+    using \<open>0 < B\<close> by (auto simp: power2_eq_square)
+  also have "(x2 - B * t)\<^sup>2 / (2 * B) = x2^2/(2*B) + B^2 * t^2/(2*B) - 2*x2*B*t/(2*B)"
+    using \<open>0 < B\<close> by (auto simp: power2_diff field_simps)
+  ultimately have "?lhs = x1 + x2\<^sup>2 / (2 * B)"
+    using \<open>0 < B\<close> by auto
+  thus "?lhs \<le> S"
+    using key by simp
+qed
+
+lemma "A > 0 \<Longrightarrow> B > 0 \<Longrightarrow> (\<lambda>s::real^3. s$2 \<ge> 0 \<and> s$1 + s$2^2/(2*B) < S) \<le>
+  |LOOP (
+    (\<lambda>s. (\<questiondown>\<lambda>s. s$1 + s$2^2/(2*B) < S?;(3 ::= (\<lambda>s. A))) s \<union> (\<questiondown>\<lambda>s. s$2 = 0?;(3 ::= (\<lambda>s. 0))) s \<union> (3 ::= (\<lambda>s. - B)) s);
+    (\<lambda>s. (x\<acute>= (\<lambda>s. \<chi> i. if i=1 then s$2 else (if i=2 then s$3 else 0)) & (\<lambda>s. s$2 \<ge> 0 \<and> s$1 + s$2^2/(2*B) \<le> S)) s \<union>
+     (x\<acute>= (\<lambda>s. \<chi> i. if i=1 then s$2 else (if i=2 then s$3 else 0)) & (\<lambda>s. s$2 \<ge> 0 \<and> s$1 + s$2^2/(2*B) \<ge> S)) s)
+  ) INV (\<lambda>s. s$2 \<ge> 0 \<and> s$1 + s$2^2/(2*B) \<le> S)]
+  (\<lambda>s. s$1 \<le> S)"
+  apply(rule fbox_loopI, simp add: le_fun_def, simp add: le_fun_def)
+   apply (smt not_sum_power2_lt_zero zero_compare_simps(5))
+  apply(simp add: fbox_choice local_flow.fbox_g_ode_subset[OF local_flow_STTT_Ex2])
+  apply(simp add: le_fun_def, safe)
+     apply(erule_tac x=0 in allE)
+  by (auto simp: STTexample3a_arith)
+
+
+subsubsection \<open> STTT Tutorial: Example 4a \<close>
+
+(* v <= V & A > 0
+ -> [
+      { {
+           ?v=V; a:=0;
+        ++ ?v!=V; a:=A;
+        }
+
+        {x' = v, v' = a & v <= V}
+      }*@invariant(v <= V)
+    ] v <= V *)
+
+lemma "A > 0 \<Longrightarrow> (\<lambda>s::real^3. s$2 \<le> V) \<le> 
+  |LOOP 
+    (\<lambda>s. (\<questiondown>\<lambda>s. s$2 = V?;(3 ::= (\<lambda>s. 0))) s \<union> (\<questiondown>\<lambda>s. s$2 \<noteq> V?;(3 ::= (\<lambda>s. A))) s);
+    (x\<acute>= (\<lambda>s. \<chi> i. if i=1 then s$2 else (if i=2 then s$3 else 0)) & (\<lambda>s. s$2 \<le> V))
+  INV (\<lambda>s. s$2 \<le> V)]
+  (\<lambda>s. s$2 \<le> V)"
+  by (rule fbox_loopI) 
+    (auto simp: fbox_choice local_flow.fbox_g_ode_subset[OF local_flow_STTT_Ex2])
+ 
+
+subsubsection \<open>STTT Tutorial: Example 4b\<close>
+
+(* v <= V & A > 0
+ -> [
+      { a := A;
+
+        {x' = v, v' = a & v <= V}
+      }*@invariant(v <= V)
+    ] v <= V *)
+lemma "A > 0 \<Longrightarrow> (\<lambda>s::real^3. s$2 \<le> V) \<le>
+  |LOOP 
+    (3 ::= (\<lambda>s. A));
+    (x\<acute>= (\<lambda>s. \<chi> i. if i=1 then s$2 else (if i=2 then s$3 else 0)) & (\<lambda>s. s$2 \<le> V))
+  INV (\<lambda>s. s$2 \<le> V)]
+  (\<lambda>s. s$2 \<le> V)"
+  by (rule fbox_loopI) 
+    (auto simp: le_fbox_choice_iff local_flow.fbox_g_ode_subset[OF local_flow_STTT_Ex2])
+ 
+
+subsubsection \<open>STTT Tutorial: Example 4c\<close>
+
+(* v <= V & A > 0
+ -> [
+      { {
+           ?v=V; a:=0;
+        ++ ?v!=V; a:=A;
+        }
+
+        {  {x' = v, v' = a & v <= V}
+        ++ {x' = v, v' = a & v >= V}}
+      }*@invariant(v <= V)
+    ] v <= V *)
+lemma "A > 0 \<Longrightarrow> (\<lambda>s::real^3. s$2 \<le> V) \<le> 
+  |LOOP 
+    (\<lambda>s. (\<questiondown>\<lambda>s. s$2 = V?;(3 ::= (\<lambda>s. 0))) s \<union> (\<questiondown>\<lambda>s. s$2 \<noteq> V?;(3 ::= (\<lambda>s. A))) s);
+    (\<lambda>s. (x\<acute>= (\<lambda>s. \<chi> i. if i=1 then s$2 else (if i=2 then s$3 else 0)) & (\<lambda>s. s$2 \<le> V)) s \<union>
+     (x\<acute>= (\<lambda>s. \<chi> i. if i=1 then s$2 else (if i=2 then s$3 else 0)) & (\<lambda>s. s$2 \<ge> V)) s)
+  INV (\<lambda>s. s$2 \<le> V)]
+  (\<lambda>s. s$2 \<le> V)"
+  apply (rule fbox_loopI) 
+    apply (simp_all add: fbox_choice local_flow.fbox_g_ode_subset[OF local_flow_STTT_Ex2])
+  by (clarsimp, erule_tac x=0 in allE, auto)
+
+
+subsubsection \<open> STTT Tutorial: Example 5 \<close>
+
+lemma STTexample5_arith:
+  assumes "0 < A" "0 < B" "0 < \<epsilon>" "0 \<le> x2" "0 \<le> (t::real)" 
+    and key: "x1 + x2\<^sup>2 / (2 * B) + (A * (A * \<epsilon>\<^sup>2 / 2 + \<epsilon> * x2) / B + (A * \<epsilon>\<^sup>2 / 2 + \<epsilon> * x2)) \<le> S" (is "?k3 \<le> S")
+    and ghyp: "\<forall>\<tau>. 0 \<le> \<tau> \<and> \<tau> \<le> t \<longrightarrow> \<tau> \<le> \<epsilon>"
+  shows "A * t\<^sup>2 / 2 + x2 * t + x1 + (A * t + x2)\<^sup>2 / (2 * B) \<le> S" (is "?k0 \<le> S")
+proof-
+  have "t \<le> \<epsilon>"
+    using ghyp \<open>0 \<le> t\<close> by auto
+  hence "A*t^2/2 + t*x2 \<le> A*\<epsilon>^2/2 + \<epsilon>*x2"
+    using \<open>0 \<le> t\<close> \<open>0 < A\<close> \<open>0 \<le> x2\<close>
+    by (smt (verit, ccfv_SIG) divide_right_mono mult_less_cancel_left mult_right_mono power_less_imp_less_base)
+  hence "((A + B)/B) * (A*t^2/2 + t*x2) + x1 + x2\<^sup>2 / (2 * B) \<le>
+    x1 + x2\<^sup>2 / (2 * B) + ((A + B)/B) * (A*\<epsilon>^2/2 + \<epsilon>*x2)" (is "?k1 \<le> ?k2")
+    using \<open>0 < B\<close> \<open>0 < A\<close> by (smt (verit, ccfv_SIG) divide_pos_pos mult_less_cancel_left) 
+  moreover have "?k0 = ?k1"
+    using \<open>0 < B\<close> \<open>0 < A\<close> by (auto simp: field_simps power2_sum power2_eq_square)
+  moreover have "?k2 = ?k3"
+    using \<open>0 < B\<close> \<open>0 < A\<close> by (auto simp: field_simps power2_sum power2_eq_square)
+  ultimately show "?k0 \<le> S"
+    using key by linarith
+qed
+
+lemma local_flow_STTT_Ex5:
+  "local_flow (\<lambda>s::real^4. \<chi> i. if i=1 then s$2 else (if i=2 then s$3 else (if i=3 then 0 else 1))) UNIV UNIV
+  (\<lambda>t s. \<chi> i. if i = 1 then s$3 * t^2/2 + s$2 * t + s$1 else (if i=2 then s$3 * t + s$2 else (if i=3 then s$3 else t+s$4)))"
+  apply(unfold_locales, simp_all add: local_lipschitz_def forall_2 lipschitz_on_def)
+    apply(clarsimp, rule_tac x=1 in exI)+
+  apply(clarsimp simp: dist_norm norm_vec_def L2_set_def)
+  unfolding UNIV_4 by (auto intro!: poly_derivatives simp: forall_4 vec_eq_iff)
+
+(* v >= 0 & A > 0 & B > 0 & x+v^2/(2*B) <= S & ep > 0
+ -> [
+      { {   ?x+v^2/(2*B) + (A/B+1)*(A/2*ep^2+ep*v) <= S; a := A;
+         ++ ?v=0; a := 0;
+         ++ a := -B;
+        };
+
+        c := 0;
+        { x' = v, v' = a, c' = 1 & v >= 0 & c <= ep }
+      }*@invariant(v >= 0 & x+v^2/(2*B) <= S)
+    ] x <= S *)
+lemma "A > 0 \<Longrightarrow> B > 0 \<Longrightarrow> \<epsilon> > 0 \<Longrightarrow> (\<lambda>s::real^4. s$2 \<ge> 0 \<and> s$1 + s$2^2/(2*B) \<le> S) \<le>
+  |LOOP 
+    (\<lambda>s.
+      (\<questiondown>\<lambda>s. s$1 + s$2^2/(2*B) + (A/B + 1) * (A/2 * \<epsilon>^2 + \<epsilon> * s$2) \<le> S?;(3 ::= (\<lambda>s. A))) s \<union> 
+      (\<questiondown>\<lambda>s. s$2 = 0?;(3 ::= (\<lambda>s. 0))) s \<union> 
+      (3 ::= (\<lambda>s. - B)) s); 
+    (4 ::= (\<lambda>s. 0));
+    (x\<acute>= (\<lambda>s. \<chi> i. if i=1 then s$2 else (if i=2 then s$3 else (if i=3 then 0 else 1))) & (\<lambda>s. s$2 \<ge> 0 \<and> s$4 \<le> \<epsilon>))
+  INV (\<lambda>s. s$2 \<ge> 0 \<and> s$1 + s$2^2/(2*B) \<le> S)]
+  (\<lambda>s. s$1 \<le> S)"
+  apply (rule fbox_loopI) 
+    apply (simp_all add: fbox_choice local_flow.fbox_g_ode_subset[OF local_flow_STTT_Ex5])
+   apply safe
+     apply (smt not_sum_power2_lt_zero zero_compare_simps(5))
+    apply(rule STTexample5_arith[of A B \<epsilon> "_ $ 2" _ "_ $ 1" S]; (simp)?)
+  by (simp add: field_simps, auto simp: STTexample3a_arith[of B _ "_ $ 2" "_ $ 1" S])
+
+
+subsubsection \<open> STTT Tutorial: Example 6 \<close>
+
+lemma STTexample6_arith:
+  assumes "0 < A" "0 < B" "0 < \<epsilon>" "0 \<le> x2" "0 \<le> (t::real)" "- B \<le> k" "k \<le> A"
+    and key: "x1 + x2\<^sup>2 / (2 * B) + (A * (A * \<epsilon>\<^sup>2 / 2 + \<epsilon> * x2) / B + (A * \<epsilon>\<^sup>2 / 2 + \<epsilon> * x2)) \<le> S" (is "?k3 \<le> S")
+    and ghyp: "\<forall>\<tau>. 0 \<le> \<tau> \<and> \<tau> \<le> t \<longrightarrow> 0 \<le> k * \<tau> + x2 \<and> \<tau> \<le> \<epsilon>"
+  shows "k * t\<^sup>2 / 2 + x2 * t + x1 + (k * t + x2)\<^sup>2 / (2 * B) \<le> S" (is "?k0 \<le> S")
+proof-
+  have "0 \<le> k * t + x2 + x2"
+    using ghyp \<open>0 \<le> x2\<close> \<open>0 \<le> t\<close> by force
+  hence "0 \<le> (k * t + 2 * x2) * t/2"
+    by (metis assms(5) divide_nonneg_pos is_num_normalize(1) mult_2 mult_sign_intros(1) rel_simps(51))
+  hence f1: "0 \<le> k*t^2/2 + t*x2"
+    by (auto simp: field_simps power2_eq_square)
+  have f2: "0 \<le> (k + B) / B" "(k + B) / B \<le> (A + B) / B"
+    using \<open>0 < A\<close> \<open>0 < B\<close> \<open>- B \<le> k\<close> \<open>k \<le> A\<close> divide_le_cancel by (auto, fastforce)
+  have "t \<le> \<epsilon>"
+    using ghyp \<open>0 \<le> t\<close> by auto
+  hence "k*t^2/2 + t*x2 \<le> A*t^2/2 + t*x2"
+    using \<open>k \<le> A\<close> by (auto simp: mult_right_mono)
+  also have f3: "... \<le> A*\<epsilon>^2/2 + \<epsilon>*x2"
+    using \<open>0 \<le> t\<close> \<open>0 < A\<close> \<open>0 \<le> x2\<close> \<open>t \<le> \<epsilon>\<close>
+    by (smt field_sum_of_halves mult_right_mono power_less_imp_less_base mult_less_cancel_left)
+  finally have "k*t^2/2 + t*x2 \<le> A*\<epsilon>^2/2 + \<epsilon>*x2" .
+  hence "((k + B)/B) * (k*t^2/2 + t*x2) \<le> ((A + B)/B) * (A*\<epsilon>^2/2 + \<epsilon>*x2)"
+    using f1 f2 \<open>k \<le> A\<close> apply(rule_tac b="((A + B)/B) * (A*t^2/2 + t*x2)" in order.trans)
+     apply (rule mult_mono', simp, simp, simp add: mult_right_mono, simp, simp)
+    by (metis f3 add_sign_intros(4) assms(1,2) less_eq_real_def mult_zero_left 
+        mult_less_cancel_left zero_compare_simps(5))
+  hence "((k + B)/B) * (k*t^2/2 + t*x2) + x1 + x2\<^sup>2 / (2 * B) \<le>
+    x1 + x2\<^sup>2 / (2 * B) + ((A + B)/B) * (A*\<epsilon>^2/2 + \<epsilon>*x2)" (is "?k1 \<le> ?k2")
+    using \<open>0 < B\<close> \<open>0 < A\<close> by (smt mult_less_cancel_left zero_compare_simps(9))
+  moreover have "?k0 = ?k1"
+    using \<open>0 < B\<close> \<open>0 < A\<close> by (auto simp: field_simps power2_sum power2_eq_square)
+  moreover have "?k2 = ?k3"
+    using \<open>0 < B\<close> \<open>0 < A\<close> by (auto simp: field_simps power2_sum power2_eq_square)
+  ultimately show "?k0 \<le> S"
+    using key by linarith
+qed
+
+(* v >= 0 & A > 0 & B > 0 & x+v^2/(2*B) <= S & ep > 0
+ -> [
+      { {   ?x+v^2/(2*B) + (A/B+1)*(A/2*ep^2+ep*v) <= S; a :=*; ?-B <= a & a <= A;
+         ++ ?v=0; a := 0;
+         ++ a := -B;
+        };
+
+        c := 0;
+        { x' = v, v' = a, c' = 1 & v >= 0 & c <= ep }
+      }*@invariant(v >= 0 & x+v^2/(2*B) <= S)
+    ] x <= S *)
+lemma "A > 0 \<Longrightarrow> B > 0 \<Longrightarrow> \<epsilon> > 0 \<Longrightarrow> (\<lambda>s::real^4. s$2 \<ge> 0 \<and> s$1 + s$2^2/(2*B) \<le> S) \<le>
+  |LOOP 
+    (\<lambda>s.
+      (\<questiondown>\<lambda>s. s$1 + s$2^2/(2*B) + (A/B + 1) * (A/2 * \<epsilon>^2 + \<epsilon> * s$2) \<le> S?;(3 ::= ?);\<questiondown>\<lambda>s. -B \<le> s$3 \<and> s$3 \<le> A?) s \<union> 
+      (\<questiondown>\<lambda>s. s$2 = 0?;(3 ::= (\<lambda>s. 0))) s \<union> 
+      (3 ::= (\<lambda>s. - B)) s); 
+    (4 ::= (\<lambda>s. 0));
+    (x\<acute>= (\<lambda>s. \<chi> i. if i=1 then s$2 else (if i=2 then s$3 else (if i=3 then 0 else 1))) & (\<lambda>s. s$2 \<ge> 0 \<and> s$4 \<le> \<epsilon>))
+  INV (\<lambda>s. s$2 \<ge> 0 \<and> s$1 + s$2^2/(2*B) \<le> S)]
+  (\<lambda>s. s$1 \<le> S)"
+  apply (rule fbox_loopI) 
+    apply (simp_all add: fbox_choice local_flow.fbox_g_ode_subset[OF local_flow_STTT_Ex5])
+   apply safe
+     apply (smt not_sum_power2_lt_zero zero_compare_simps(5))
+    apply(rule STTexample6_arith[of A B \<epsilon> "_$2" _ _ "_$1"]; simp?)
+  by (force simp: field_simps, auto simp: STTexample3a_arith STTexample6_arith)
+
+
+subsubsection \<open> STTT Tutorial: Example 7 \<close>
+
+lemma STTexample7_arith1:
+  assumes "(0::real) < A" "0 < b" "0 < \<epsilon>" "0 \<le> v" "0 \<le> t" "k \<le> A"
+    and "x + v\<^sup>2 / (2 * b) + (A * (A * \<epsilon>\<^sup>2 / 2 + \<epsilon> * v) / b + (A * \<epsilon>\<^sup>2 / 2 + \<epsilon> * v)) \<le> S" (is "?expr1 \<le> S")
+    and guard: "\<forall>\<tau>. 0 \<le> \<tau> \<and> \<tau> \<le> t \<longrightarrow> 0 \<le> k * \<tau> + v \<and> \<tau> \<le> \<epsilon>"
+  shows "k * t\<^sup>2 / 2 + v * t + x + (k * t + v)\<^sup>2 / (2 * b) \<le> S" (is "?lhs \<le> S")
+proof-
+  have obs1: "?lhs*(2*b) = k*t\<^sup>2*b + 2 * v * t*b + 2*x*b + (k*t+v)\<^sup>2" (is "_ = ?expr2 k t")
+    using \<open>0 < b\<close> by (simp add: field_simps)
+  have "?expr2 A \<epsilon> = ?expr1*(2*b)"
+    using \<open>0 < b\<close> by (simp add: field_simps power2_eq_square)
+  also have "... \<le> S*(2*b)"
+    using \<open>?expr1 \<le> S\<close> \<open>0 < b\<close> by force 
+  finally have obs2: "?expr2 A \<epsilon> \<le> S*(2*b)" .
+  have "t \<le> \<epsilon>"
+    using guard \<open>0 \<le> t\<close> by auto
+  hence "t\<^sup>2 \<le> \<epsilon>\<^sup>2" "k * t + v \<le> A * \<epsilon> + v"
+    using \<open>k \<le> A\<close> \<open>0 < A\<close> power_mono[OF \<open>t \<le> \<epsilon>\<close> \<open>0 \<le> t\<close>, of 2] 
+    by auto (meson \<open>0 \<le> t\<close> less_eq_real_def mult_mono)
+  hence "k * t\<^sup>2 * b \<le> A * \<epsilon>\<^sup>2 * b" "2 * v * t * b \<le> 2 * v * \<epsilon> * b"
+    using \<open>t \<le> \<epsilon>\<close> \<open>0 < b\<close> \<open>k \<le> A\<close> \<open>0 \<le> v\<close> 
+    by (auto simp: mult_left_mono) (meson \<open>0 < A\<close> less_eq_real_def mult_mono zero_compare_simps(12))
+  hence "?expr2 k t \<le> ?expr2 A \<epsilon>"
+    by (smt \<open>k * t + v \<le> A * \<epsilon> + v\<close> ends_in_segment(2) \<open>0 \<le> t\<close> guard power_mono)
+  hence "?lhs*(2*b) \<le> S*(2*b)" 
+    using obs1 obs2 by simp
+  thus "?lhs \<le> S"
+    using \<open>0 < b\<close> by force
+qed
+
+lemma STTexample7_arith2:
+  assumes "(0::real) < b" "0 \<le> v" "0 \<le> t" "k \<le> - b"
+    and key: "x + v\<^sup>2 / (2 * b) \<le> S" 
+    and guard: "\<forall>\<tau>. 0 \<le> \<tau> \<and> \<tau> \<le> t \<longrightarrow> 0 \<le> k * \<tau> + v \<and> \<tau> \<le> \<epsilon>"
+  shows "k * t\<^sup>2 / 2 + v * t + x + (k * t + v)\<^sup>2 / (2 * b) \<le> S" (is "?lhs \<le> S")
+proof-
+  have obs: "1 + k/b \<le> 0" "k * t + v \<ge> 0"
+    using \<open>k \<le> - b\<close> \<open>0 < b\<close> guard \<open>0 \<le> t\<close> by (auto simp: mult_imp_div_pos_le real_add_le_0_iff)
+  have "?lhs = (k * t + v + v)*t/2 * (1 + k/b) + x + v\<^sup>2 / (2 * b)"
+    using \<open>0 < b\<close> by (auto simp: field_simps power2_eq_square)
+  also have "... \<le> x + v\<^sup>2 / (2 * b)"
+    using obs \<open>0 \<le> t\<close> \<open>0 \<le> v\<close>
+    by (smt mult_nonneg_nonneg zero_compare_simps(11) zero_compare_simps(6))
+  also have "... \<le> S"
+    using key .
+  finally show ?thesis .
+qed
+
+(* v >= 0 & A > 0 & B >= b & b > 0 & x+v^2/(2*b) <= S & ep > 0
+ -> [
+      { {   ?x+v^2/(2*b) + (A/b+1)*(A/2*ep^2+ep*v) <= S; a :=*; ?-B <= a & a <= A;
+         ++ ?v=0; a := 0;
+         ++ a :=*; ?-B <=a & a <= -b;
+        };
+
+        c := 0;
+        { x' = v, v' = a, c' = 1 & v >= 0 & c <= ep }
+      }*@invariant(v >= 0 & x+v^2/(2*b) <= S)
+    ] x <= S *)
+lemma "A > 0 \<Longrightarrow> B \<ge> b \<Longrightarrow> b > 0 \<Longrightarrow> \<epsilon> > 0 \<Longrightarrow> (\<lambda>s::real^4. s$2 \<ge> 0 \<and> s$1 + s$2^2/(2*b) \<le> S) \<le> 
+  |LOOP 
+    (\<lambda>s. 
+      (\<questiondown>\<lambda>s. s$1 + s$2^2/(2*b) + (A/b + 1) * (A/2 * \<epsilon>^2 + \<epsilon> * s$2) \<le> S?;(3 ::= ?);\<questiondown>\<lambda>s. -B \<le> s$3 \<and> s$3 \<le> A?) s \<union> 
+      (\<questiondown>\<lambda>s. s$2 = 0?;(3 ::= (\<lambda>s. 0))) s \<union> 
+      ((3 ::= ?);\<questiondown>\<lambda>s. -B \<le> s$3 \<and> s$3 \<le> - b?) s
+    );(4 ::= (\<lambda>s. 0));
+    (x\<acute>= (\<lambda>s. \<chi> i. if i=1 then s$2 else (if i=2 then s$3 else (if i=3 then 0 else 1))) & (\<lambda>s. s$2 \<ge> 0 \<and> s$4 \<le> \<epsilon>))
+  INV (\<lambda>s. s$2 \<ge> 0 \<and> s$1 + s$2^2/(2*b) \<le> S)]
+  (\<lambda>s. s$1 \<le> S)"
+  apply (rule fbox_loopI) 
+    apply (simp_all add: fbox_choice local_flow.fbox_g_ode_subset[OF local_flow_STTT_Ex5])
+   apply(safe)
+     apply (smt not_sum_power2_lt_zero zero_compare_simps(5))
+    apply(rule STTexample7_arith1[of A b \<epsilon> "_$2" _ _ "_$1" S]; simp?)
+  apply(force simp: field_simps, force)
+  using STTexample7_arith2[of b "_$2" _ _ "_$1" S] by blast
+
+
+subsubsection \<open> STTT Tutorial: Example 9a \<close>
+
+lemma STTexample9a_arith:
+  "(10*x-10*r) * v/4 + v\<^sup>2/2 + (x-r)*(2*r-2*x-3 * v)/2 + v * (2*r-2*x-3 * v)/2 \<le> (0::real)" 
+  (is "?t1 + ?t2 + ?t3 + ?t4 \<le> 0")
+proof-
+  have "?t1 = 5 * (x-r) * v/2"
+    by auto
+  moreover have "?t3 = -((x - r)^2) - 3 * v * (x-r)/2"
+    by (auto simp: field_simps power2_diff power2_eq_square)
+  moreover have "?t4 = - 2 * (x - r) * v/2 - 3 * v^2/2"
+    by (auto simp: field_simps power2_diff power2_eq_square)
+  ultimately have "?t1 + ?t3 + ?t4 = -((x - r)^2) - 3 * v^2/2"
+    by (auto simp: field_simps)
+  hence "?t1 + ?t2 + ?t3 + ?t4 = -((x - r)^2) - v^2"
+    by auto
+  also have "... \<le> 0"
+    by auto
+  finally show ?thesis .
+qed
+
+(* v >= 0 & c() > 0 & Kp() = 2 & Kd() = 3 & 5/4*(x-xr())^2 + (x-xr())*v/2 + v^2/4 < c()
+ -> [
+      { x' = v, v' = -Kp()*(x-xr()) - Kd()*v }
+    ] 5/4*(x-xr())^2 + (x-xr())*v/2 + v^2/4 < c() *)
+lemma "c > 0 \<Longrightarrow> Kp = 2 \<Longrightarrow> Kd = 3 \<Longrightarrow> (\<lambda>s::real^2. (5/4)*(s$1-xr)^2 + (s$1-xr)*(s$2)/2 + (s$2)^2/4 < c) \<le> 
+  |x\<acute>= (\<lambda>s. \<chi> i. if i=1 then s$2 else -Kp*(s$1-xr) - Kd*(s$2) ) & G]
+  (\<lambda>s. (5/4)*(s$1-xr)^2 + (s$1-xr)*(s$2)/2 + (s$2)^2/4 < c)"
+  apply(simp, rule_tac \<mu>'="\<lambda>s. 0" and \<nu>'="\<lambda>s. 10*(s$1-xr)*(s$2)/4 + (s$2^2)/2 + 
+    (s$1-xr)*(-Kp*(s$1-xr)-Kd*(s$2))/2 + (s$2)*(-Kp*(s$1-xr)-Kd*(s$2))/2" in diff_invariant_rules(3); 
+      clarsimp simp: forall_2 STTexample9a_arith)
+  apply(intro poly_derivatives; (rule poly_derivatives)?)
+  by force+ (auto simp: field_simps power2_eq_square)
+
+
+subsubsection \<open> STTT Tutorial: Example 9b \<close> (*N 50 *)
+
+ (* require differentiable \<Longrightarrow> lipschitz *)
+
+(* v >= 0 & xm <= x & x <= S & xr = (xm + S)/2 & Kp = 2 & Kd = 3
+           & 5/4*(x-xr)^2 + (x-xr)*v/2 + v^2/4 < ((S - xm)/2)^2
+ -> [ { {  xm := x;
+           xr := (xm + S)/2;
+           ?5/4*(x-xr)^2 + (x-xr)*v/2 + v^2/4 < ((S - xm)/2)^2;
+        ++ ?true;
+        };
+        {{ x' = v, v' = -Kp*(x-xr) - Kd*v & v >= 0 }
+          @invariant(
+            xm<=x,
+            5/4*(x-(xm+S())/2)^2 + (x-(xm+S())/2)*v/2 + v^2/4 < ((S()-xm)/2)^2
+         )
+        }
+      }*@invariant(v >= 0 & xm <= x & xr = (xm + S)/2 & 5/4*(x-xr)^2 + (x-xr)*v/2 + v^2/4 < ((S - xm)/2)^2)
+    ] x <= S *)
+
+
+subsubsection \<open> STTT Tutorial: Example 10 \<close> (*N 51 *)
+
+(*
+ v >= 0 & A > 0 & B >= b & b > 0 & ep > 0 & lw > 0 & y = ly & r != 0 & dx^2 + dy^2 = 1
+           & abs(y-ly) + v^2/(2*b) < lw
+ -> [
+      { {   ?abs(y-ly) + v^2/(2*b) + (A/b+1)*(A/2*ep^2+ep*v) < lw;
+            a :=*; ?-B <= a & a <= A;
+            w :=*; r :=*; ?r != 0 & w*r = v;
+         ++ ?v=0; a := 0; w := 0;
+         ++ a :=*; ?-B <=a & a <= -b;
+        }
+
+        c := 0;
+        {
+        { x' = v*dx, y' = v*dy, v' = a, dx' = -dy*w, dy' = dx*w, w'=a/r, c' = 1 & v >= 0 & c <= ep }
+        @invariant(c>=0, dx^2+dy^2=1,
+          (v'=a -> v=old(v)+a*c),
+          (v'=a -> -c*(v-a/2*c) <= y - old(y) & y - old(y) <= c*(v-a/2*c)),
+          (v'=0 -> v=old(v)),
+          (v'=0 -> -c*v <= y - old(y) & y - old(y) <= c*v)
+        )
+        }
+      }*@invariant(v >= 0 & dx^2+dy^2 = 1 & r != 0 & abs(y-ly) + v^2/(2*b) < lw)
+    ] abs(y-ly) < lw *)
+
+subsubsection \<open> LICS: Example 1 Continuous car accelerates forward \<close>
+
+(*
+   v>=0 & a>=0
+ -> [
+      {x'=v, v'=a & v>=0}
+    ] v>=0 *)
+lemma "(\<lambda>s::real^3. s$2 \<ge> 0 \<and> s$3 \<ge> 0) \<le>
+  |x\<acute>= (\<lambda>s. \<chi> i. if i=1 then s$2 else (if i=2 then s$3 else 0)) & (\<lambda>s. s$2 \<ge> 0)]
+  (\<lambda>s. s$2 \<ge> 0)"
+  by (simp_all add: local_flow.fbox_g_ode_subset[OF local_flow_STTT_Ex2], simp add: le_fun_def)
+ 
+
+subsubsection \<open> LICS: Example 2 Single car drives forward \<close>
+
+(* v>=0  & A>=0 & b>0
+ -> [
+      {
+        {a:=A; ++ a:=-b;}
+        {x'=v, v'=a & v>=0}
+      }*@invariant(v>=0)
+    ] v>=0 *)
+lemma "A \<ge> 0 \<Longrightarrow> b > 0 \<Longrightarrow> (\<lambda>s::real^3. s$2 \<ge> 0) \<le>
+  |LOOP
+    (\<lambda>s. (3 ::= (\<lambda>s. A)) s \<union> (3 ::= (\<lambda>s. -b)) s);
+    (x\<acute>= (\<lambda>s. \<chi> i. if i=1 then s$2 else (if i=2 then s$3 else 0)) & (\<lambda>s. s$2 \<ge> 0))
+  INV (\<lambda>s. s$2 \<ge> 0)]
+  (\<lambda>s. s$2 \<ge> 0)"
+  apply (rule fbox_loopI) 
+  by (simp_all add: local_flow.fbox_g_ode_subset[OF local_flow_STTT_Ex2] fbox_choice)
+    (simp add: le_fun_def)
+
+subsubsection \<open> LICS: Example 3a event-triggered car drives forward \<close>
+
+(*
+( v >= 0
+	 & A >= 0
+	 & b > 0 )
+->
+  [
+    {
+      {  ?(m-x>=2); a := A;
+      ++ a := -b;
+      };
+      {x' = v, v' = a & v >= 0}
+    }*@invariant(v >= 0)
+  ]v >= 0 *)
+lemma "A \<ge> 0 \<Longrightarrow> b > 0 \<Longrightarrow> (\<lambda>s::real^3. s$2 \<ge> 0) \<le>
+  |LOOP
+    (\<lambda>s. (\<questiondown>\<lambda>s. m - s$1 \<ge> 2?;(3 ::= (\<lambda>s. A))) s \<union> (3 ::= (\<lambda>s. -b)) s);
+    (x\<acute>= (\<lambda>s. \<chi> i. if i=1 then s$2 else (if i=2 then s$3 else 0)) & (\<lambda>s. s$2 \<ge> 0))
+  INV (\<lambda>s. s$2 \<ge> 0)]
+  (\<lambda>s. s$2 \<ge> 0)"
+  apply (rule fbox_loopI) 
+  by (simp_all add: local_flow.fbox_g_ode_subset[OF local_flow_STTT_Ex2] fbox_choice)
+    (simp add: le_fun_def)
+
+
+subsubsection \<open> LICS: Example 4a safe stopping of time-triggered car \<close>
+
+lemma LICSexample4a_arith:
+  assumes "(0::real) \<le> A" "0 < b" "v\<^sup>2 \<le> 2 * b * (m - x)" "0 \<le> t"
+      and guard: "\<forall>\<tau>. 0 \<le> \<tau> \<and> \<tau> \<le> t \<longrightarrow> 0 \<le> A * \<tau> + v \<and> \<tau> \<le> \<epsilon>"
+      and key: "v\<^sup>2 + (A * (A * \<epsilon>\<^sup>2 + 2 * \<epsilon> * v) + b * (A * \<epsilon>\<^sup>2 + 2 * \<epsilon> * v)) \<le> 2 * b * (m - x)" (is "?expr1 \<le> _")
+    shows "(A * t + v)\<^sup>2 \<le> 2 * b * (m - (A * t\<^sup>2 / 2 + v * t + x))"
+proof-
+  have "t \<le> \<epsilon>" "0 \<le> v"
+    using guard \<open>0 \<le> t\<close> by (force, erule_tac x=0 in allE, auto)
+  hence "A * t\<^sup>2 + 2 * t * v \<le> A * \<epsilon>\<^sup>2 + 2 * \<epsilon> * v"
+    using \<open>0 \<le> A\<close> \<open>0 \<le> t\<close>
+    by (smt mult_less_cancel_left_disj mult_right_mono power_less_imp_less_base) 
+  hence "v\<^sup>2 + (A + b) * (A * t\<^sup>2 + 2 * t * v) \<le> v\<^sup>2 + (A + b) * (A * \<epsilon>\<^sup>2 + 2 * \<epsilon> * v)"
+    using \<open>0 \<le> A\<close> \<open>0 < b\<close> by (smt mult_left_mono) 
+  also have "... = ?expr1"
+    by (auto simp: field_simps)
+  finally have "v\<^sup>2 + (A + b) * (A * t\<^sup>2 + 2 * t * v) \<le> 2 * b * (m - x)"
+    using key by auto
+  thus ?thesis
+    by (auto simp: field_simps power2_eq_square)
+qed
+
+(*v^2<=2*b*(m-x) & v>=0  & A>=0 & b>0
+ -> [
+      {
+        {?(2*b*(m-x) >= v^2+(A+b)*(A*ep^2+2*ep*v)); a:=A; ++ a:=-b; }
+        t := 0;
+        {x'=v, v'=a, t'=1 & v>=0 & t<=ep}
+      }*@invariant(v^2<=2*b*(m-x))
+    ] x <= m *)
+lemma "A \<ge> 0 \<Longrightarrow> b > 0 \<Longrightarrow> (\<lambda>s::real^4. s$2^2 \<le> 2*b*(m-s$1) \<and> s$2 \<ge> 0) \<le>
+  |LOOP
+    (\<lambda>s. (\<questiondown>\<lambda>s. 2*b*(m-s$1) \<ge> s$2^2+(A+b)*(A*\<epsilon>\<^sup>2+2*\<epsilon>*(s$2))?;(3 ::= (\<lambda>s. A))) s \<union> (3 ::= (\<lambda>s. -b)) s);
+    (4 ::= (\<lambda>s. 0));
+    (x\<acute>= (\<lambda>s. \<chi> i. if i=1 then s$2 else (if i=2 then s$3 else (if i=3 then 0 else 1))) & (\<lambda>s. s$2 \<ge> 0 \<and> s$4 \<le> \<epsilon>))
+  INV (\<lambda>s. s$2^2 \<le> 2*b*(m-s$1))]
+  (\<lambda>s. s$1 \<le> m)"
+  apply (rule fbox_loopI) 
+    apply (simp_all add: fbox_choice local_flow.fbox_g_ode_subset[OF local_flow_STTT_Ex5])
+   apply(safe, smt not_sum_power2_lt_zero zero_compare_simps(10))
+  apply(rule LICSexample4a_arith[of A b "_$2" m "_$1" _ \<epsilon>]; simp?)
+   apply(force simp: field_simps)
+  by (auto simp: power2_diff power2_eq_square[symmetric] algebra_simps(18,19) 
+      mult.assoc[symmetric] power_mult_distrib)
+
+
+subsubsection \<open> LICS: Example 4b progress of time-triggered car \<close>  (*N 56 *)
+
+(* ep() > 0 & A() > 0 & b() > 0
+->
+  \forall p \exists m
+  <
+    {
+        {?(2*b()*(m-x) >= v^2+(A()+b())*(A()*ep()^2+2*ep()*v)); a:=A(); ++ a:=-b(); }
+        t := 0;
+        {x'=v, v'=a, t'=1 & v>=0 & t<=ep()}
+    }*
+  > (x >= p) *)
+
+
+subsubsection \<open> LICS: Example 4c relative safety of time-triggered car \<close>
+
+lemma in_fbox_loopI: 
+  "I s \<Longrightarrow> I \<le> Q \<Longrightarrow> I \<le> |R] I \<Longrightarrow> ( |LOOP R INV I] Q) s"
+  using fbox_loopI[of I I Q R] by auto
+
+abbreviation LICS_Ex4c_f :: "real \<Rightarrow> real \<Rightarrow> real^4 \<Rightarrow> real^4" ("f")
+  where "f time acc s \<equiv> (\<chi> i. if i=1 then s$2 else (if i=2 then acc else if i=3 then 0 else time))"
+
+lemma local_flow_LICS_Ex4c_1:
+  "local_flow (f k a) UNIV UNIV
+  (\<lambda>t s. \<chi> i. if i=1 then a * t^2/2 + s$2 * t + s$1 else 
+             (if i=2 then a * t + s$2               else 
+             (if i=3 then s$3                       else 
+                          k * t + s$4               )))"
+  apply(unfold_locales, simp_all add: local_lipschitz_def forall_2 lipschitz_on_def)
+    apply(clarsimp, rule_tac x=1 in exI)+
+  apply(clarsimp simp: dist_norm norm_vec_def L2_set_def)
+  unfolding UNIV_4 by (auto intro!: poly_derivatives simp: forall_4 vec_eq_iff)
+
+lemma local_flow_LICS_Ex4c_2:
+  "local_flow (\<lambda>s. f k (s$3) s) UNIV UNIV
+  (\<lambda>t s. \<chi> i. if i=1 then s$3 * t^2/2 + s$2 * t + s$1 else 
+             (if i=2 then s$3 * t + s$2               else 
+             (if i=3 then s$3                       else 
+                          k * t + s$4               )))"
+  apply(unfold_locales, simp_all add: local_lipschitz_def forall_2 lipschitz_on_def)
+    apply(clarsimp, rule_tac x=1 in exI)+
+  apply(clarsimp simp: dist_norm norm_vec_def L2_set_def)
+  unfolding UNIV_4 by (auto intro!: poly_derivatives simp: forall_4 vec_eq_iff)
+
+lemma LICSexample4c_arith1:
+  assumes "v\<^sup>2 \<le> 2 * b * (m - x)" "0 \<le> t" "A \<ge> 0" "b > 0"
+    and key: "v\<^sup>2 + (A * (A * \<epsilon>\<^sup>2 + 2 * \<epsilon> * v) + b * (A * \<epsilon>\<^sup>2 + 2 * \<epsilon> * v)) \<le> 2 * b * (m - x)"
+    and guard: "\<forall>\<tau>. 0 \<le> \<tau> \<and> \<tau> \<le> t \<longrightarrow> (0::real) \<le> A * \<tau> + v \<and> \<tau> \<le> \<epsilon>"
+  shows "(A * t + v)\<^sup>2 \<le> 2 * b * (m - (A * t\<^sup>2 / 2 + v * t + x))" (is "_ \<le> ?rhs")
+proof-
+  have "t \<le> \<epsilon>" "0 \<le> \<epsilon>" "0 \<le> v"
+    using guard \<open>0 \<le> t\<close> by (force, erule_tac x=0 in allE, simp, erule_tac x=0 in allE, simp)
+  hence obs1: "A * t\<^sup>2 + 2 * t * v \<le> A * \<epsilon>\<^sup>2 + 2 * \<epsilon> * v"
+    using \<open>A \<ge> 0\<close> \<open>0 \<le> t\<close> \<open>t \<le> \<epsilon>\<close> by (smt mult_mono power_mono zero_compare_simps(12)) 
+  have obs2:"?rhs + A * b * t^2 + 2 * b * v * t = 2 * b * (m - x)"
+    by (simp add: field_simps)
+  have "(A * t + v)\<^sup>2 + A * b * t^2 + 2 * b * v * t = v\<^sup>2 + (A * (A * t\<^sup>2 + 2 * t * v) + b * (A * t\<^sup>2 + 2 * t * v))"
+    by (simp add: field_simps power2_eq_square)
+  also have "... \<le> v\<^sup>2 + (A * (A * \<epsilon>\<^sup>2 + 2 * \<epsilon> * v) + b * (A * \<epsilon>\<^sup>2 + 2 * \<epsilon> * v))"
+    using obs1 \<open>A \<ge> 0\<close> \<open>b > 0\<close> by (smt mult_less_cancel_left) 
+  also have "... \<le> 2 * b * (m - x)"
+    using key .
+  finally show ?thesis
+    using obs2 by auto
+qed
+
+(* ( [{x' = v, v' = -b()}]x<=m()
+   & v >= 0
+	 & A() >= 0
+	 & b() > 0 )
+->
+  [
+    {
+      {  ?(2*b()*(m()-x) >= v^2 + (A() + b())*(A()*ep()^2 + 2*ep()*v)); a := A();
+      ++ a := -b();
+      };
+      t := 0;
+      {x' = v, v' = a, t' = 1 & v >= 0 & t <= ep()}
+    }*@invariant(v^2<=2*b()*(m()-x))
+  ]x<=m() *)
+
+lemma 
+  assumes "A \<ge> 0" "b > 0" "s$2 \<ge> 0"
+  shows "( |x\<acute>=(f 0 (-b)) & (\<lambda>s. True)] (\<lambda>s. s$1 \<le> m)) s \<Longrightarrow> 
+  ( |LOOP
+    (\<lambda>s. (\<questiondown>\<lambda>s. 2*b*(m-s$1) \<ge> s$2^2+(A+b)*(A*\<epsilon>^2+2*\<epsilon>*(s$2))?;(3 ::= (\<lambda>s. A))) s \<union> (3 ::= (\<lambda>s. -b)) s);
+    (4 ::= (\<lambda>s. 0));
+    (x\<acute>= (\<lambda>s. f 1 (s$3) s) & (\<lambda>s. s$2 \<ge> 0 \<and> s$4 \<le> \<epsilon>))
+  INV (\<lambda>s. s$2^2 \<le> 2*b*(m-s$1))] (\<lambda>s. s$1 \<le> m)) s"
+  apply(subst (asm) local_flow.fbox_g_ode_subset[OF local_flow_LICS_Ex4c_1], simp_all)
+  apply(rule in_fbox_loopI)
+     apply(erule_tac x="s$2/b" in allE)
+  using \<open>b > 0\<close> \<open>s$2 \<ge> 0\<close> apply(simp add: field_simps power2_eq_square)
+   apply (simp add: le_fun_def, smt \<open>b > 0\<close> mult_sign_intros(6) sum_power2_ge_zero)
+  apply(simp add: fbox_choice)
+  apply(simp_all add: local_flow.fbox_g_ode_subset[OF local_flow_LICS_Ex4c_2], safe)
+  apply(rule LICSexample4c_arith1[OF _ _ \<open>0 \<le> A\<close> \<open>0 < b\<close>, of "_$2" m "_$1" _ \<epsilon>]; simp?)
+  by (auto simp: field_simps power2_eq_square)
+
+no_notation LICS_Ex4c_f ("f")
+
+
+subsubsection \<open> LICS: Example 5 Controllability Equivalence \<close>
+
+lemma LICSexample5_arith1:
+  assumes "(0::real) < b" "0 \<le> t"
+    and key: "v\<^sup>2 \<le> 2 * b * (m - x)"
+  shows "v * t - b * t\<^sup>2 / 2 + x \<le> m"
+proof-
+  have "v\<^sup>2 \<le> 2 * b * (m - x) + (b * t - v)^2"
+    using key by (simp add: add_increasing2) 
+  hence "b^2 * t^2 - 2 * b * v * t \<ge> 2 * b * x - 2 * b * m"
+    by (auto simp: field_simps power2_diff)
+  hence "(b^2/b) * t^2 - 2 * (b/b) * v * t \<ge> 2 * (b/b) * x - 2 * (b/b) * m"
+    using \<open>b > 0\<close> by (auto simp: field_simps)
+  thus ?thesis
+    using \<open>b > 0\<close> by (simp add: power2_eq_square)
+qed
+
+lemma LICSexample5_arith2:
+  assumes "(0::real) < b" "0 \<le> v" "\<forall>t\<in>{0..}. v * t - b * t\<^sup>2 / 2 + x \<le> m"
+  shows "v\<^sup>2 \<le> 2 * b * (m - x)"
+proof(cases "v = 0")
+  case True
+  have "m - x \<ge> 0"
+    using assms by (erule_tac x=0 in ballE, auto)
+  thus ?thesis 
+    using assms True by auto
+next
+  case False
+  hence obs: "v > 0 \<and> (\<exists>k. k > 0 \<and> v = b * k)"
+    using assms(1,2) by (metis (no_types, hide_lams) divide_pos_pos divide_self_if 
+        less_eq_real_def linorder_not_le mult_1_right mult_1s(1) times_divide_eq_left) 
+  {fix t::real assume "t \<ge> 0"
+    hence "v * t - b * t\<^sup>2 / 2 + x \<le> m"
+      using assms by auto
+    hence "2 * b * v * t - b * b * t\<^sup>2 + 2 * b * x \<le> 2 * b * m"
+      using \<open>b > 0\<close> by (simp add: field_simps) (metis distrib_left mult_le_cancel_left_pos) 
+    hence "- b\<^sup>2 * t\<^sup>2 + 2 * b * v * t \<le> 2 * b * m - 2 * b * x"
+      using \<open>b > 0\<close> by (simp add: power2_eq_square) 
+    hence "v^2 \<le> 2 * b * (m - x) + (b^2 * t^2 + v^2 - 2 * b * v * t)"
+      by (simp add: field_simps)
+    also have "... = 2 * b * (m - x) + (b * t - v)^2"
+      by (simp add: power2_diff power_mult_distrib)
+    finally have "v^2 \<le> 2 * b * (m - x) + (b * t - v)^2" .}
+  hence "\<forall>t\<ge>0. v\<^sup>2 \<le> 2 * b * (m - x) + (b * t - v)\<^sup>2"
+    by blast
+  then obtain k where "v\<^sup>2 \<le> 2 * b * (m - x) + (b * k - v)\<^sup>2 \<and> k > 0 \<and> v = b * k"
+    using obs by fastforce
+  then show ?thesis 
+    by auto
+qed
+
+(* v>=0 & b>0 -> ( v^2<=2*b*(m-x) <-> [{x'=v, v'=-b}]x<=m ) *)
+lemma "b > 0 \<Longrightarrow> (s::real^2)$2 \<ge> 0 \<Longrightarrow> 
+   s$2^2 \<le> 2*b*(m-s$1) \<longleftrightarrow> ( |x\<acute>= (\<lambda>s. \<chi> i. if i=1 then s$2 else -b) & (\<lambda>s. True)] (\<lambda>s. s$1 \<le> m)) s"
+  apply(subst local_flow.fbox_g_ode_subset[where T="UNIV" 
+        and \<phi>="\<lambda>t s. \<chi> i::2. if i=1 then -b * t^2/2 + s$2 * t + s$1 else -b * t + s$2"])
+      apply(unfold_locales, simp_all add: local_lipschitz_def forall_2 lipschitz_on_def)
+     apply(clarsimp simp: dist_norm norm_vec_def L2_set_def, rule_tac x=1 in exI)+
+  unfolding UNIV_2 apply clarsimp
+  apply(force intro!: poly_derivatives)
+  using exhaust_2 apply(force simp: vec_eq_iff)
+  by (auto simp: LICSexample5_arith1 LICSexample5_arith2)
+
+
+subsubsection \<open> LICS: Example 6 MPC Acceleration Equivalence \<close>  (*N 59 *)
+
+lemma LICSexample6_arith1:
+  assumes "0 \<le> v" "0 < b" "0 \<le> A" "0 \<le> \<epsilon>" and guard: "\<forall>t\<in>{0..}. (\<forall>\<tau>. 0 \<le> \<tau> \<and> \<tau> \<le> t \<longrightarrow> \<tau> \<le> \<epsilon>) \<longrightarrow> (\<forall>\<tau>\<in>{0..}. 
+  A * t * \<tau> + v * \<tau> - b * \<tau>\<^sup>2 / 2 + (A * t\<^sup>2 / 2 + v * t + x) \<le> (m::real))"
+  shows "v\<^sup>2 + (A * (A * \<epsilon>\<^sup>2 + 2 * \<epsilon> * v) + b * (A * \<epsilon>\<^sup>2 + 2 * \<epsilon> * v)) \<le> 2 * b * (m - x)"
+proof-
+  {fix \<tau>::real
+    assume "\<tau> \<ge> 0"
+    hence "A * \<epsilon> * \<tau> + v * \<tau> - b * \<tau>\<^sup>2 / 2 + (A * \<epsilon>\<^sup>2 / 2 + v * \<epsilon> + x) \<le> m"
+      using guard \<open>0 \<le> \<epsilon>\<close> apply(erule_tac x=\<epsilon> in ballE)
+      by (erule impE, auto simp: closed_segment_eq_real_ivl)
+    hence "2 * (A * \<epsilon> * \<tau> + v * \<tau> - b * \<tau>\<^sup>2 / 2 + (A * \<epsilon>\<^sup>2 / 2 + v * \<epsilon> + x)) * b \<le> 2 * m * b"
+      using \<open>0 < b\<close> by (meson less_eq_real_def mult_left_mono mult_right_mono rel_simps(51)) 
+    hence "2 * A * \<epsilon> * \<tau> * b + 2 * v * \<tau> * b - b^2 * \<tau>\<^sup>2 + b * (A * \<epsilon>\<^sup>2 + 2 * v * \<epsilon>) \<le> 2 * b * (m - x)"
+      using \<open>0 < b\<close> apply(simp add: algebra_simps(17,18,19,20) add.assoc[symmetric] 
+          power2_eq_square[symmetric] mult.assoc[symmetric])
+      by (simp add: mult.commute mult.left_commute power2_eq_square)}
+  hence "\<forall>\<tau>\<ge>0. 2 * A * \<epsilon> * \<tau> * b + 2 * v * \<tau> * b - b^2 * \<tau>\<^sup>2 + b * (A * \<epsilon>\<^sup>2 + 2 * v * \<epsilon>) \<le> 2 * b * (m - x)"
+    by blast
+  moreover have "2 * A * \<epsilon> * ((A*\<epsilon> + v)/b) * b + 2 * v * ((A*\<epsilon> + v)/b) * b - b^2 * ((A*\<epsilon> + v)/b)\<^sup>2 =
+    2 * A * \<epsilon> * (A*\<epsilon> + v) + 2 * v * (A*\<epsilon> + v) - (A*\<epsilon> + v)\<^sup>2"
+    using \<open>0 < b\<close> by (simp add: field_simps)
+  moreover have "... = v\<^sup>2 + A * (A * \<epsilon>\<^sup>2 + 2 * \<epsilon> * v)"
+    using \<open>0 < b\<close> by (simp add: field_simps power2_eq_square)
+  moreover have "(A*\<epsilon> + v)/b \<ge> 0"
+    using assms by auto
+  ultimately have "v\<^sup>2 + A * (A * \<epsilon>\<^sup>2 + 2 * \<epsilon> * v) + b * (A * \<epsilon>\<^sup>2 + 2 * v * \<epsilon>) \<le> 2 * b * (m - x)"
+    using assms by (erule_tac x="(A*\<epsilon> + v)/b" in allE, auto)
+  thus ?thesis
+    by argo
+qed
+
+
+lemma LICSexample6_arith2:
+  assumes "0 \<le> v" "0 < b" "0 \<le> A" "0 \<le> t" "0 \<le> \<tau>" "t \<le> \<epsilon>"
+    and "v\<^sup>2 + (A * (A * \<epsilon>\<^sup>2 + 2 * \<epsilon> * v) + b * (A * \<epsilon>\<^sup>2 + 2 * \<epsilon> * v)) \<le> 2 * b * (m - x)"
+  shows "A * \<epsilon> * \<tau> + s $ 2 * \<tau> - b * \<tau>\<^sup>2 / 2 + (A * \<epsilon>\<^sup>2 / 2 + s $ 2 * \<epsilon> + s $ 1) \<le> m"
+  (* Need to show that function (\<lambda>\<tau>. A * \<epsilon> * \<tau> + s $ 2 * \<tau> - b * \<tau>\<^sup>2 / 2) attains maximum at \<tau> = (A*\<epsilon> + v)/b *)
+  oops
+
+lemma local_flow_LICS_Ex6:
+  "local_flow (\<lambda>s::real^3. \<chi> i. if i=1 then s$2 else (if i=2 then k1 else k2)) UNIV UNIV
+  (\<lambda>t s. \<chi> i. if i = 1 then k1 * t^2/2 + s$2 * t + s$1 else (if i=2 then k1 * t + s$2 else k2 * t + s$3))"
+  apply(unfold_locales, simp_all add: local_lipschitz_def forall_2 lipschitz_on_def)
+    apply(clarsimp, rule_tac x=1 in exI)+
+  apply(clarsimp simp: dist_norm norm_vec_def L2_set_def)
+  unfolding UNIV_3 by (auto intro!: poly_derivatives simp: forall_3 vec_eq_iff)
+
+(* v>=0 & b>0 & A>=0 & ep>=0 -> (
+    [t:=0; {x'=v, v'=A, t'=1 & t<=ep}][{x'=v, v'=-b}]x<=m
+    <->
+    2*b*(m-x) >= v^2 + (A + b)*(A*ep^2 + 2*ep*v)
+   ) *)
+lemma "s$2 \<ge> 0 \<Longrightarrow> b>0 \<Longrightarrow> A \<ge> 0 \<Longrightarrow> \<epsilon> \<ge> 0 \<Longrightarrow>  
+  ( |(3 ::= (\<lambda>s. 0));
+    (x\<acute>= (\<lambda>s::real^3. \<chi> i. if i=1 then s$2 else (if i=2 then A else 1)) & (\<lambda>s. s$3 \<le> \<epsilon>))]
+  |x\<acute>= (\<lambda>s. \<chi> i. if i=1 then s$2 else (if i=2 then -b else 0)) & (\<lambda>s. True)] (\<lambda>s. s$1 \<le> m)) s
+\<longleftrightarrow>
+  2*b*(m-s$1) \<ge> s$2^2+(A+b)*(A*\<epsilon>^2+2*\<epsilon>*(s$2))"
+  apply (simp add: le_fbox_choice_iff local_flow.fbox_g_ode_subset[OF local_flow_LICS_Ex6], safe)
+  apply(subst Groups.algebra_simps(17))
+   apply(rule LICSexample6_arith1[of "_$2" b A \<epsilon> "_$1" m]; simp?)
+   apply(force simp: field_simps)
+  apply(erule_tac x=t in allE; clarsimp)
+  apply(rename_tac t \<tau>)
+  apply(rule_tac b="A * \<epsilon> * \<tau> + s $ 2 * \<tau> - b * \<tau>\<^sup>2 / 2 + (A * \<epsilon>\<^sup>2 / 2 + s $ 2 * \<epsilon> + s $ 1)" in order.trans)
+   apply(simp add: algebra_simps)
+  (* using LICSexample6_arith2 *)
+  oops
+
+
+subsubsection \<open> LICS: Example 7 Model-Predictive Control Design Car \<close>  (*N 60 *)
+
+notation LICS_Ex4c_f ("f")
+
+(* [{x'=v, v'=-b}](x<=m)
+   & v >= 0
+   & A >= 0
+   & b > 0
+->
+  [
+    {
+    {{?([t:=0; {x'=v, v'=A, t'=1 & v >= 0 & t<=ep}] [{x'=v, v'=-b}](x<=m));
+       a := A;}
+    ++ a := -b;}
+      t := 0;
+      {x'=v, v'=a, t'=1 & v>=0 & t<=ep}
+    }*@invariant([{x'=v, v'=-b}](x<=m))
+  ] (x <= m) *)
+
+lemma "( |x\<acute>=(f 0 (-b)) & (\<lambda>s. True)] (\<lambda>s. s$1 \<le> m)) s \<Longrightarrow> s$2 \<ge> 0 \<Longrightarrow> A \<ge> 0 \<Longrightarrow> b > 0 \<Longrightarrow> 
+  ( |LOOP (
+  (\<lambda>s. (\<questiondown>|(3 ::= (\<lambda>s. 0));(x\<acute>= (f 1 A) & (\<lambda>s. s$2 \<ge> 0 \<and> s$4 \<le> \<epsilon>))] |x\<acute>= (f 0 (-b)) & (\<lambda>s. True)] (\<lambda>s. s$1 \<le> m)?;
+  (3 ::= (\<lambda>s. A))) s \<union> 
+  (3 ::= (\<lambda>s. -b)) s); 
+  (4 ::= (\<lambda>s. 0)); 
+  (x\<acute>= (\<lambda>s. f 1 (s$3) s) & (\<lambda>s. s$2 \<ge> 0 \<and> s$4 \<le> \<epsilon>))
+  ) INV (\<lambda>s. ( |x\<acute>=(f 1 (-b)) & (\<lambda>s. True)] (\<lambda>s. s$1 \<le> m)) s)] (\<lambda>s. s$1 \<le> m)) s"
+  apply(rule in_fbox_loopI, simp_all add: local_flow.fbox_g_ode_subset[OF local_flow_LICS_Ex4c_1]
+      local_flow.fbox_g_ode_subset[OF local_flow_LICS_Ex4c_2] le_fbox_choice_iff, safe)
+      apply(erule_tac x=0 in allE, erule_tac x=0 in allE, simp)
+  oops
+
+
+no_notation LICS_Ex4c_f ("f")
+
+
+subsection \<open>Advanced\<close>
+
+
+subsubsection \<open> ETCS: Essentials \<close>
+
+locale ETCS =
+  fixes \<epsilon> b A m::real
+(* Real ep; /* Control cycle duration upper bound */
+   Real b;  /* Braking force */
+   Real A;  /* Maximum acceleration */
+   Real m;  /* End of movement authority (train must not drive past m) *)
+begin
+
+(* Real stopDist(Real v) = v^2/(2*b) *)
+abbreviation "stopDist v \<equiv> v^2/(2*b)"
+
+(* Real accCompensation(Real v) = (((A/b) + 1)*((A/2)*ep^2 + ep*v)) *)
+abbreviation "accCompensation v \<equiv> ((A/b) + 1) * ((A/2)*\<epsilon>^2 + \<epsilon> * v)"
+
+(* Real SB(Real v) = stopDist(v) + accCompensation(v) *)
+abbreviation "SB v \<equiv> stopDist v + accCompensation v"
+
+(* initial(Real m, Real z, Real v) <-> (v >= 0 & m-z >= stopDist(v) & b>0 & A>=0 & ep>=0) *)
+abbreviation "initial m' z v \<equiv> (v \<ge> 0 \<and> (m' - z) \<ge> stopDist v)" (* Initial states *)
+
+(* Bool safe(Real m, Real z, Real v, Real d) <-> (z >= m -> v <= d) *)
+abbreviation "safe m' z v \<delta> \<equiv> z \<ge> m' \<longrightarrow> v \<le> \<delta>" 
+
+(* Bool loopInv(Real m, Real z, Real v) <-> (v >= 0 & m-z >= stopDist(v) *)
+abbreviation "loopInv m' z v \<equiv> v \<ge> 0 \<and> m' - z \<ge> stopDist v" (* always maintain sufficient stopping distance *)
+
+(*HP ctrl ::= {?m - z <= SB(v); a := -b; ++ ?m - z >= SB(v); a :=  A; *)
+abbreviation "ctrl s \<equiv> (\<questiondown>\<lambda>s::real^4. m - s$1 \<le> SB (s$2)?;(3 ::= (\<lambda>s. -b))) s \<union> 
+ (\<questiondown>\<lambda>s. m - s$1 \<ge> SB (s$2)?;(3 ::= (\<lambda>s. A))) s" (* train controller *)
+
+(* HP drive ::= {t := 0;{z'=v, v'=a, t'=1  & v >= 0 & t <= ep} *)
+abbreviation "drive \<equiv> (4 ::= (\<lambda>s. 0));
+  (x\<acute>= (\<lambda>s::real^4. \<chi> i. if i=1 then s$2 else (if i=2 then s$3 else (if i=3 then 0 else 1))) 
+  & (\<lambda>s. s$2 \<ge> 0 \<and> s$4 \<le> \<epsilon>))"
+
+lemma ETCS_arith1: 
+  assumes "0 < b" "0 \<le> A" "0 \<le> v" "0 \<le> t"
+    and "v\<^sup>2 / (2 * b) + (A * (A * \<epsilon>\<^sup>2 / 2 + \<epsilon> * v)/ b + (A * \<epsilon>\<^sup>2 / 2 + \<epsilon> * v)) \<le> m - x" (is "?expr1 \<le> m - x")
+    and guard: "\<forall>\<tau>. 0 \<le> \<tau> \<and> \<tau> \<le> t \<longrightarrow> \<tau> \<le> \<epsilon>"
+  shows "(A * t + v)\<^sup>2/(2 * b) \<le> m - (A * t\<^sup>2/2 + v * t + x)" (is "?lhs \<le> ?rhs")
+proof-
+  have "2*b*(v\<^sup>2/(2*b) + (A*(A*\<epsilon>\<^sup>2/2+\<epsilon>* v)/b + (A*\<epsilon>\<^sup>2/2+\<epsilon>* v))) \<le> 2*b*(m-x)" (is "?expr2 \<le> 2*b*(m-x)")
+    using \<open>0 < b\<close> mult_left_mono[OF \<open>?expr1 \<le> m - x\<close>, of "2 * b"] by auto
+  also have "?expr2 = v\<^sup>2 +  2 * A * (A * \<epsilon>\<^sup>2 / 2 + \<epsilon> * v) + b * A * \<epsilon>\<^sup>2 + 2 * b * \<epsilon> * v"
+    using \<open>0 < b\<close> by (auto simp: field_simps)
+  also have "... = v\<^sup>2 +  A^2 * \<epsilon>\<^sup>2 + 2 * A * \<epsilon> * v + b * A * \<epsilon>\<^sup>2 + 2 * b * \<epsilon> * v"
+    by (auto simp: field_simps power2_eq_square)
+  finally have obs: "v\<^sup>2 +  A\<^sup>2*\<epsilon>\<^sup>2 + 2*A*\<epsilon>* v + b*A*\<epsilon>\<^sup>2 + 2*b*\<epsilon>* v \<le> 2*b*(m-x)" (is "?expr3 \<epsilon> \<le> 2*b*(m-x)") .
+  have "t \<le> \<epsilon>"
+    using guard \<open>0 \<le> t\<close> by auto
+  hence "v\<^sup>2 + A\<^sup>2 * t\<^sup>2 + b * A * t\<^sup>2 \<le> v\<^sup>2 + A\<^sup>2 * \<epsilon>\<^sup>2 + b * A * \<epsilon>\<^sup>2"
+    using power_mono[OF \<open>t \<le> \<epsilon>\<close> \<open>0 \<le> t\<close>, of 2]
+    by (smt assms(1,2) mult_less_cancel_left zero_compare_simps(4) zero_le_power) 
+  hence "v\<^sup>2 + A\<^sup>2 * t\<^sup>2 + 2 * A * t * v + b * A * t\<^sup>2 \<le> v\<^sup>2 + A\<^sup>2 * \<epsilon>\<^sup>2 + 2 * A * \<epsilon> * v + b * A * \<epsilon>\<^sup>2"
+    using assms(1,2,3,4) \<open>t \<le> \<epsilon>\<close> by (smt mult_left_mono mult_right_mono) 
+  hence "?expr3 t \<le> 2 * b * (m - x)"
+    using assms(1,2,3,4) \<open>t \<le> \<epsilon>\<close> obs
+    by (smt (z3) mult_less_cancel_left mult_minus_right mult_right_mono_neg) 
+  hence "A\<^sup>2 * t\<^sup>2 + v\<^sup>2 + 2 * A * t * v \<le> 2 * b * m - b * A * t\<^sup>2 - 2 * b * t * v - 2 * b * x"
+    by (simp add: right_diff_distrib)
+  hence "(A * t + v)\<^sup>2 \<le> 2 * b * m - b * A * t\<^sup>2 - 2 * b * t * v - 2 * b * x"
+    unfolding cross3_simps(29)[of A t 2] power2_sum[of "A*t" v] by (simp add: mult.assoc)
+  hence "?lhs \<le> (2 * b * m - b * A * t\<^sup>2 - 2 * b * t * v - 2 * b * x)/(2 * b)" (is "_ \<le> ?expr4")
+    using \<open>0 < b\<close> divide_right_mono by fastforce
+  also have "?expr4 = ?rhs"
+    using \<open>0 < b\<close> by (auto simp: field_simps)
+  finally show "?lhs \<le> ?rhs" .
+qed
+
+(* Safety specification of the form: initial -> [{ctrl;plant}*]safe *)
+lemma "b > 0 \<Longrightarrow> A \<ge> 0 \<Longrightarrow> \<epsilon> \<ge> 0 \<Longrightarrow> 
+  (\<lambda>s. initial m (s$1) (s$2)) \<le> |LOOP ctrl;drive INV (\<lambda>s. loopInv m (s$1) (s$2))] (\<lambda>s. s$1 \<le> m)"
+  apply (rule fbox_loopI)
+    apply (simp_all add: le_fbox_choice_iff local_flow.fbox_g_ode_subset[OF local_flow_STTT_Ex5], safe)
+    apply (smt divide_le_cancel divide_minus_left not_sum_power2_lt_zero)
+   apply(auto simp: field_simps power2_eq_square)[1]
+  by (rule ETCS_arith1[of "_$2" _ "_$1"], auto simp: field_simps)
+
+subsection \<open> ETCS: Proposition 1 (Controllability) \<close> (*N 62 *)
+
+(* Bool Assumptions(Real v, Real d) <-> ( v>=0 & d>=0 & b>0 ) *)
+abbreviation "assumptions v \<delta> \<equiv> (v \<ge> 0 \<and> \<delta> \<ge> 0 \<and> b > 0)" 
+
+lemma ETCS_Prop1_arith1:
+  assumes "0 \<le> v" "0 \<le> \<delta>" "0 < b" "x \<le> m"
+    and "\<forall>t\<in>{0..}. (\<forall>\<tau>\<in>{0--t}. b * \<tau> \<le> v) \<longrightarrow>
+       m \<le> v * t - b * t\<^sup>2 / 2 + x \<longrightarrow> v - b * t \<le> \<delta>"
+  shows "v\<^sup>2 - \<delta>\<^sup>2 \<le> 2 * b * (m - x)"
+    (* solve arithmetic *)
+  sorry
+
+lemma ETCS_Prop1_arith2:
+  assumes "0 \<le> v" "0 \<le> \<delta>" "0 < b" "x \<le> m" "0 \<le> t"
+      and key: "v\<^sup>2 - \<delta>\<^sup>2 \<le> 2 * b * (m - x)" "m \<le> v * t - b * t\<^sup>2 / 2 + x"
+      and guard: "\<forall>\<tau>\<in>{0--t}. b * \<tau> \<le> v"
+    shows "v - b * t \<le> \<delta>"
+proof-
+  have "2 * b * (m - x) \<le> 2 * b * (v * t - b * t\<^sup>2 / 2) - v\<^sup>2 + v\<^sup>2"
+    using key(2) \<open>0 < b\<close> by simp
+  also have "... = v\<^sup>2 - (v - b * t)\<^sup>2"
+    using \<open>0 < b\<close> by (simp add: power2_diff field_simps power2_eq_square)
+  finally have "(v - b * t)\<^sup>2 \<le> \<delta>\<^sup>2"
+    using key(1) by simp
+  thus "v - b * t \<le> \<delta>"
+    using guard \<open>0 \<le> t\<close> \<open>0 \<le> \<delta>\<close> by auto
+qed
+
+(* Assumptions(v, d) & z<=m
+  ->
+  ( [ {z'=v, v'=-b & v>=0 } ](z>=m -> v<=d)
+    <->
+    v^2-d^2 <= 2*b*(m-z)
+  ) *)
+lemma "assumptions (s$2) \<delta> \<and> (s$1) \<le> m \<Longrightarrow> 
+  ( |x\<acute>= (\<lambda>t s::real^2. \<chi> i. if i=1 then (s$2) else -b) & (\<lambda>s. s$2 \<ge> 0) on (\<lambda>s. {0..}) UNIV @ 0]
+  (\<lambda>s. s$1 \<ge> m \<longrightarrow> s$2 \<le> \<delta>)) s \<longleftrightarrow> s$2^2 - \<delta>^2 \<le> 2*b*(m-s$1)"
+  apply(subst local_flow.fbox_g_ode_subset[where T="UNIV" 
+        and \<phi>="\<lambda>t s. \<chi> i::2. if i=1 then -b * t^2/2 + s$2 * t + s$1 else -b * t + s$2"])
+      apply(unfold_locales, simp_all add: local_lipschitz_def forall_2 lipschitz_on_def)
+     apply(clarsimp simp: dist_norm norm_vec_def L2_set_def, rule_tac x=1 in exI)+
+  unfolding UNIV_2 using exhaust_2 
+  by (auto intro!: poly_derivatives simp: vec_eq_iff 
+      ETCS_Prop1_arith1 closed_segment_eq_real_ivl ETCS_Prop1_arith2)
+
+
+subsection \<open> ETCS: Proposition 4 (Reactivity) \<close> (*N 63 *)
+
+(* Bool Assumptions(Real v, Real d) <-> ( v>=0 & d>=0 & b>0 ) *)
+term "assumptions v \<delta>"
+
+(* Bool Controllable(Real m, Real z, Real v, Real d) <-> (v^2-d^2 <= 2*b*(m-z) & Assumptions(v, d)) *)
+abbreviation "controllable m' z v \<delta> \<equiv> v^2 - \<delta>^2 \<le> 2 * b * (m' - z) \<and> assumptions v \<delta>"
+
+(* HP drive ::= {t := 0;{z'=v, v'=a, t'=1  & v >= 0 & t <= ep}} *)
+term "drive"
+
+(* em = 0 & d >= 0 & b > 0 & ep > 0 & A > 0 & v>=0
+  -> ((\<forall> m \<forall> z (m-z>= sb & Controllable(m,z,v,d) -> [ a:=A; drive; ]Controllable(m,z,v,d)) )
+      <->
+      sb >= (v^2 - d^2) /(2*b) + (A/b + 1) * (A/2 * ep^2 + ep*v)) *)
+lemma "\<delta> \<ge> 0 \<and> b > 0 \<and> \<epsilon> > 0 \<and> A > 0 \<and> s$2 \<ge> 0 \<Longrightarrow> 
+ (\<forall>m. \<forall>z. m - s$1 \<ge> sb \<and> controllable m (s$1) (s$2) \<delta> \<longrightarrow> ( |(3 ::= (\<lambda>s. A));drive] (\<lambda>s. controllable m (s$1) (s$2) \<delta>)) s)
+  \<longleftrightarrow> sb \<ge> (s$2\<^sup>2 - \<delta>\<^sup>2)/(2*b) + (A/b + 1) * (A/2 * \<epsilon>\<^sup>2 + \<epsilon> * (s$2))"
+  apply (simp_all add: local_flow.fbox_g_ode_subset[OF local_flow_STTT_Ex5])
+  apply(rule iffI, safe)
+  oops
+
+end
+
+(*
+% 10 unsolved problems
+% 3 basic need sorry in arithmetic
+% 1 advanced need sorry in arithmetic
+% 1 basic has been solved with evol
+% 1 advanced does not match Isabelle syntax
+% 2 basic did not even try
+% 1 basic is diamond
+% 1 basic requires change of interval
+*)
+
+end
